theories/iris_system/syn_invariants.v
@@ -1,5 +1,5 @@
 From stdpp Require Import coPset gmap namespaces.
-From iris Require Import bi.big_op.
+From iris Require Import bi.big_op coPset.
 From iris.proofmode Require Import proofmode.
 Require Export Coqlib own SAT sProp invariants.
 
@@ -7,15 +7,19 @@ Local Notation level := nat.
 
 (* Syntactic invariants *)
 Variant inv_ops : Type :=
-| _ownI (u : univ_id) (i : positive)
-| _ownI_auth (u : univ_id) (keys : gmap positive unit)
-| _wsat_auth (u : univ_id).
+| _ownI (i : positive)
+| _ownI_reserve (X : coPset)
+| _ownD (i : positive)
+(* | _ownI_auth (keys : gmap positive unit) *)
+| _wsat_auth (X : coPset).
 
 Local Definition inv_arity (op : inv_ops) (sProp : Type) : Type :=
   match op with
-  | _ownI u i => fin 1
-  | _ownI_auth u keys => positive
-  | _wsat_auth u => fin 0
+  | _ownI i => fin 1
+  | _ownI_reserve X => fin 0
+  | _ownD i => fin 1
+  (* | _ownI_auth keys => positive *)
+  | _wsat_auth X => fin 0
   end.
 
 Global Instance inv_syntax : SAT.t := {
@@ -25,12 +29,15 @@ Global Instance inv_syntax : SAT.t := {
 
 (* Invariant interpretations *)
 Local Definition inv_interp_aux `{!invG Γ Σ α, !subG Γ Σ} n (op : inv_ops) :
-    (inv_arity op (GTerm.t_prev n) → GTerm.t n) → (inv_arity op (GTerm.t_prev n) → iProp Σ)
-    → iProp Σ :=
+    (inv_arity op (GTerm.t_prev n) → GTerm.t n) →
+    (inv_arity op (GTerm.t_prev n) → iProp Σ) →
+    iProp Σ :=
   match op with
-  | _ownI u i => λ syn _, ownI u n i (syn 0%fin)
-  | _ownI_auth u keys => λ syn _, ownI_auth u n (map_imap (λ k v, Some (syn k)) keys)
-  | _wsat_auth u => λ _ _, wsat_auth u n
+  | _ownI i => λ syn _, ownI i (syn 0%fin)
+  | _ownI_reserve X => λ _ _, ownI_reserve n X
+  | _ownD i => λ syn _, ownD i (syn 0%fin)
+  (* | _ownI_auth keys => λ syn _, ownI_auth n (map_imap (λ k v, Some (syn k)) keys) *)
+  | _wsat_auth X => λ _ _, wsat_auth n X
   end.
 
 Global Instance inv_interp `{!invG Γ Σ α, !subG Γ Σ} :
@@ -44,45 +51,49 @@ Class syn_invG (Γ : HRA) (Σ : GRA) (α : GAT.t) (β : GATIntp.t) (τ : TypG.t)
 
 Section syn_inv.
   Context `{!invG Γ Σ α, !subG Γ Σ, !STτ.t τ, !SL.G Γ Σ α β τ, !syn_invG Γ Σ α β τ}.
-  Local Existing Instances invG_I invG_E invG_D.
+  Local Existing Instances invG_I invG_E.
 
-  Local Definition syn_ownI u n i (p : GTerm.t n) : GTerm.t n :=
-    ⟨ _ownI u i, λ _, p ⟩.
-  Local Definition syn_ownI_auth u n (I : gmap positive (GTerm.t n)) : GTerm.t n :=
-    ⟨ _ownI_auth u (gset_to_gmap tt (dom I)), λ i, or_else (I !! i) emp%SAT⟩.
-  Local Definition syn_wsat_auth u n : GTerm.t n :=
-    ⟨ _wsat_auth u, λ e, match e with end ⟩.
+  Local Definition syn_ownI {n} i (p : GTerm.t n) : GTerm.t n :=
+    ⟨ _ownI i, λ _, p ⟩.
+  Local Definition syn_ownI_reserve {n} X : GTerm.t n :=
+    ⟨ _ownI_reserve X, λ e, match e with end⟩.
+  Local Definition syn_ownD {n} i (p : GTerm.t n) : GTerm.t n :=
+    ⟨ _ownD i, λ _, p ⟩.
+  (* Local Definition syn_ownI_auth u n (I : gmap positive (GTerm.t n)) : GTerm.t n :=
+    ⟨ _ownI_auth u (gset_to_gmap tt (dom I)), λ i, or_else (I !! i) emp%SAT⟩. *)
+  Local Definition syn_wsat_auth n X : GTerm.t n :=
+    ⟨ _wsat_auth X, λ e, match e with end ⟩.
 
-  Local Definition syn_ownE (u : univ_id) n (E : coPset) : GTerm.t n :=
-    <own> base_γ (ownER u E).
-  Local Definition syn_ownD (u : univ_id) n (D : gset positive) : GTerm.t n :=
+  Local Definition syn_ownE n (E : coPset) : GTerm.t n :=
+    <own> base_γ (CoPset E).
+  (* Local Definition syn_ownD n (D : gset positive) : GTerm.t n :=
     <own> base_γ (ownDR u D).
-  Local Definition syn_ownD_auth (u : univ_id) n : GTerm.t n :=
-    (∃ D : τ{⇣gset positive}, <own> base_γ (ownD_authR u D))%SAT.
+  Local Definition syn_ownD_auth n : GTerm.t n :=
+    (∃ D : τ{⇣gset positive}, <own> base_γ (ownD_authR u D))%SAT. *)
 
-  Local Definition syn_inv_satall u n (I : gmap positive (GTerm.t n)) : GTerm.t n :=
-    ([∗ n map] i ↦ p ∈ I, (p ∗ syn_ownD u n {[i]}) ∨ syn_ownE u n {[i]})%SAT.
-  Local Definition syn_wsat u n : GTerm.t (S n) :=
-    (∃ I : τ{ST.gmapT Φ}, (⤉ syn_ownI_auth u n I) ∗ (⤉ syn_inv_satall u n I))%SAT.
+  Local Definition syn_inv_satall {n} (I : gmap positive (GTerm.t n)) : GTerm.t n :=
+    ([∗ n map] i ↦ p ∈ I, syn_ownI i p ∗ ((syn_ownD i p ∗ p) ∨ syn_ownE n {[i]}))%SAT.
+  Local Definition syn_wsat n X : GTerm.t (S n) :=
+    (∃ I : τ{ST.gmapT Φ}, let dom := gset_to_coPset (dom I) in
+      ⌜dom ⊆ X⌝ ∗ (⤉ syn_inv_satall I) ∗ (⤉ syn_ownI_reserve (X ∖ dom)))%SAT.
 
-  Local Fixpoint syn_wsatl u n : GTerm.t n :=
+  Local Fixpoint syn_wsatl n X : GTerm.t n :=
     match n with
     | O => emp%SAT
-    | S n' => syn_wsat u n' ∗ ⤉ syn_wsatl u n'
+    | S n' => syn_wsat n' X ∗ ⤉ syn_wsatl n' X
     end.
-  Local Definition syn_wsats u n (E : coPset) : GTerm.t n :=
-    syn_wsat_auth u n ∗ syn_ownE u n E ∗ syn_ownD_auth u n ∗ syn_wsatl u n.
+  Local Definition syn_wsats n (E : coPset) : GTerm.t n :=
+    syn_wsat_auth n E ∗ syn_wsatl n E.
 
   (* Interface for the user *)
-  Local Definition syn_inv_def (u : univ_id) (n : level) (N : namespace) p :=
-    (∃ i : τ{⇣positive}, ⌜i ∈ (↑N : coPset)⌝ ∧ syn_ownI u n i p)%SAT.
+  Local Definition syn_inv_def {n : level} (N : namespace) (p : GTerm.t n) :=
+    (∃ i : τ{⇣positive}, ⌜i ∈ (↑N : coPset)⌝ ∧ syn_ownI i p)%SAT.
   Local Definition syn_inv_aux : seal (@syn_inv_def). Proof using. by eexists. Qed.
   Definition syn_inv := syn_inv_aux.(unseal).
   Local Definition syn_inv_eq : @syn_inv = @syn_inv_def := syn_inv_aux.(seal_eq).
 
-  Local Definition syn_fupd_def u b (E1 E2 : coPset) (P : GTerm.t b) : GTerm.t b :=
-    syn_wsatl u b ∗ syn_ownE u b E1 ∗ syn_ownD_auth u b
-    ==∗ (syn_wsatl u b ∗ syn_ownE u b E2 ∗ syn_ownD_auth u b ∗ P).
+  Local Definition syn_fupd_def {n} (Ew E1 E2 : coPset) (P : GTerm.t n) : GTerm.t n :=
+    syn_wsatl n Ew ∗ syn_ownE n E1 ==∗ (syn_wsatl n Ew ∗ syn_ownE n E2 ∗ P).
   Local Definition syn_fupd_aux : seal (@syn_fupd_def). Proof using. by eexists. Qed.
   Definition syn_fupd := syn_fupd_aux.(unseal).
   Local Definition syn_fupd_eq : @syn_fupd = @syn_fupd_def := syn_fupd_aux.(seal_eq).
@@ -98,8 +109,8 @@ Class sinvG (Γ : HRA) (Σ : GRA) (α : GAT.t) (β : GATIntp.t) (τ : TypG.t)
 Section reduction.
   Context `{!sinvG Γ Σ α β τ _I _S}.
 
-  Lemma ownI_auth_red u n I :
-    ⟦syn_ownI_auth u n I⟧ = ownI_auth u n I.
+  (* Lemma ownI_auth_red n I :
+    ⟦syn_ownI_auth n I⟧ = ownI_auth n I.
   Proof using.
     SAT_red; ss.
     f_equal. apply map_eq; intros i.
@@ -110,25 +121,27 @@ Section reduction.
     { rewrite map_lookup_imap lookup_gset_to_gmap //=. case_guard; ss.
       rewrite not_elem_of_dom_1; eauto.
     }
-  Qed.
-
-  Lemma wsat_red u n : ⟦syn_wsat u n⟧ ≡ wsat u n.
+  Qed. *)
+  Implicit Types (n : level) (X : coPset).
+  Lemma wsat_red n X : ⟦syn_wsat n X⟧ ≡ wsat n X.
   Proof using.
     rewrite /syn_wsat /wsat; SAT_red; SL_red.
     iSplit; iIntros "[%I H]"; SL_red.
-    { rewrite @SATRed.lift ownI_auth_red. SAT_red. rewrite /syn_inv_satall; SL_red.
-      iExists I; iDestruct "H" as "[$ H]".
+    { rewrite ?@SATRed.lift. SAT_red. rewrite /syn_inv_satall; SL_red.
+      iExists I; iDestruct "H" as "[$ [H $]]".
       rewrite /inv_satall. iApply (big_sepM_mono with "H"); ss.
-      rewrite /ownD /ownE. intros k x IN; SL_red; ss.
+      intros k x IN; SL_red; SAT_red; ss.
+      iIntros "[$ [[??]|$]]"; iLeft; iFrame.
     }
-    { iExists I; SL_red; rewrite !@SATRed.lift ownI_auth_red /syn_inv_satall; SL_red.
-      iDestruct "H" as "[$ H]".
-      rewrite /inv_satall. iApply (big_sepM_mono with "H"); ss.
-      rewrite /ownD /ownE. intros k x IN; SL_red; ss.
+    { iExists I; SL_red; SAT_red.
+      iDestruct "H" as "[$ [H $]]".
+      rewrite /syn_inv_satall; SL_red. iApply (big_sepM_mono with "H"); ss.
+      intros k x IN; SL_red; SAT_red; ss.
+      iIntros "[$ [[??]|$]]"; iLeft; iFrame.
     }
   Qed.
 
-  Lemma wsatl_red u n : ⟦syn_wsatl u n⟧ ≡ wsatl u n.
+  Lemma wsatl_red n X : ⟦syn_wsatl n X⟧ ≡ wsatl n X.
   Proof using.
     induction n.
     { SAT_red; SL_red; ss. }
@@ -138,27 +151,24 @@ Section reduction.
     }
   Qed.
   
-  Lemma wsats_red u n E : ⟦syn_wsats u n E⟧ ≡ wsats u n E.
+  Lemma wsats_red n E : ⟦syn_wsats n E⟧ ≡ wsats n E.
   Proof using.
-    rewrite /syn_wsats /syn_ownE /syn_ownD_auth. SAT_red. SL_red.
+    rewrite /syn_wsats /syn_ownE. SAT_red. SL_red.
     rewrite wsatl_red; SAT_red; ss; rewrite /wsats /ownD_auth.
-    iSplit; iIntros "($ & $ & [%x H] & $)"; iExists x; SL_red; iFrame.
   Qed.
 
-  Lemma inv_red u n N p : ⟦syn_inv u n N p⟧ ≡ inv u n N p.
+  Lemma inv_red n N p : ⟦syn_inv n N p⟧ ≡ inv n N p.
   Proof using.
     rewrite syn_inv_eq /syn_inv_def. SL_red.
     rewrite /inv invariants.inv_aux.(seal_eq) /invariants.inv_def.
     iSplit; iIntros "[%x H]"; iExists x; SL_red; SAT_red; ss.
   Qed.
 
-  Lemma fupd_red u n E1 E2 P : ⟦syn_fupd u n E1 E2 P⟧ ≡ uPred_fupd u n E1 E2 ⟦P⟧.
+  Lemma fupd_red n Ew E1 E2 P : ⟦syn_fupd n Ew E1 E2 P⟧ ≡ uPred_fupd n Ew E1 E2 ⟦P⟧.
   Proof using.
     rewrite syn_fupd_eq /uPred_fupd invariants.uPred_fupd_aux.(seal_eq) /invariants.uPred_fupd_def.
     rewrite /syn_fupd_def SLRed.wand SLRed.upd. repeat SAT_red.
-    rewrite wsatl_red /wsatl /syn_ownE /syn_ownD_auth; SL_red.
-    iSplit; iIntros "I [W [E [%x D]]]"; iMod ("I" with "[W E D]") as "[$ [$ [[%x' I] $]]]"; SL_red; iFrame.
-    all: ss; iExists _; SL_red; ss.
+    rewrite wsatl_red /wsatl /syn_ownE; SL_red. done.
   Qed.
 End reduction.
 
@@ -211,5 +221,4 @@ Module inv_instances.
 
   #[export] Instance subGH_app_r (Σ: GRA) (Γ1 : HRA) (Σ2 : GRA) : subG Σ Σ2 → subG Σ (GRAs.app Γ1 Σ2).
   Proof using. move=> H i; move: H=> /(_ i) [j ?]. exists (Fin.R _ j). by rewrite /= fin_add_inv_r. Defined.
-  
 End inv_instances.
