theories/simulations/wsim/WSim.v
@@ -1,5 +1,5 @@
-Require Import Common.
 From iris.proofmode Require Import proofmode.
+Require Import Common.
 Require Import ISim SMod SModTr HMod HModSim.
 Require Import TacticsCommon.
 
@@ -8,15 +8,18 @@ From stdpp Require Import coPset.
 Section FSPEC.
   Context `{!sinvG Γ Σ α β τ _I _S}.
 
-  Definition wsim_ginv (u : univ_id) (E : coPset): iProp Σ :=
-    own_admin ∗ (∃ n, univs u n) ∗ (∃ n, wsats u n E).
+  Definition wsim_ginv (Ep : option (coPset * coPset)): iProp Σ :=
+    match Ep with
+    | Some (Ew, E) => own_admin ∗ ownE E ∗ (∃ n, wsats n Ew)
+    | None => emp
+    end.
 
-  Definition wsim_fspec (υ : univ_id) (fsp : fspec) : fspec :=
+  Definition fspec_wsim (E : coPset) (fsp : fspec) : fspec :=
     mk_fspec (meta := fsp.(meta))
-      (λ x varg arg, wsim_ginv υ ⊤ ∗ fsp.(precond) x varg arg)%I
-      (λ x vret ret, wsim_ginv υ ⊤ ∗ fsp.(postcond) x vret ret)%I.
+      (λ x varg arg, wsim_ginv (Some (E, E)) ∗ fsp.(precond) x varg arg)%I
+      (λ x vret ret, wsim_ginv (Some (E, E)) ∗ fsp.(postcond) x vret ret)%I.
 
-  Lemma wsim_ginv_split (υ ν : univ_id) (E : coPset):
+  (* Lemma wsim_ginv_split (υ ν : univ_id) (E : coPset):
     (ν < υ) →
     wsim_ginv υ E
     ==∗ wsim_ginv ν ⊤ ∗ own_admin ∗ (∃ n, wsats υ n E) ∗ (wsim_ginv ν ⊤ ==∗ ∃ n, univs υ n).
@@ -32,13 +35,12 @@ Section FSPEC.
     iPoseProof (wsats_mon ν n' n'' with "W") as "> W"; first lia.
     iFrame. iApply big_sepL_bupd. iApply (big_sepL_impl with "U3").
     iModIntro; iIntros "%k %x %IN W"; iApply wsats_mon; last iFrame; lia.
-  Qed.
+  Qed. *)
 End FSPEC.
 
-Class WP `{!sinvG Γ Σ α β τ _I _G} 
-    (P : iProp Σ) (υ : univ_id) (E : coPset) := mk_WP {
+Class WP `{!sinvG Γ Σ α β τ _I _G} (P : iProp Σ) (Ew E : coPset) := mk_WP {
   WP_remainder : iProp Σ;
-  WP_iff : P ∗-∗ wsim_ginv υ E ∗ WP_remainder
+  WP_iff : P ∗-∗ wsim_ginv (Some (Ew, E)) ∗ WP_remainder
 }.
 Arguments mk_WP {_ _ _ _ _ _ _ _} _ _ _ _ _.
 Arguments WP_remainder {_ _ _ _ _ _ _ _} [_ _ _] _.
@@ -52,87 +54,83 @@ Section wsim.
   Local Definition rel : Type := ∀ R_s R_t : Type,
     post R_s R_t → bool → bool → nat → state * itree hmodE R_s → state * itree hmodE R_t → iProp Σ.
 
-  Implicit Types r g : rel.
+  (* Implicit Types r g : rel.
   Implicit Types ps pt : bool.
   Implicit Types nths : nat.
-  Implicit Types E : coPset.
+  Implicit Types E : coPset. *)
 
   (* TODO : abstraction into mixins *)
-  (* TODO : hard-code nodup conditions *)
+  (* Local Definition wsim_pre Ep : iProp Σ :=
+    wsim_ginv  
   Local Definition wsim_pre t υ ν E : iProp Σ :=
     match t with
     | None => True
     | Some false => own_admin ∗ (∃ n, wsats υ n E) ∗ (wsim_ginv ν ⊤ ==∗ ∃ n, univs υ n)
     | Some true => wsim_ginv υ E
-    end.
+    end. *)
 
-  Definition wsim_rel t υ ν E (r : rel) : rel :=
+  (* Definition wsim_rel t υ ν E (r : rel) : rel :=
     λ R_s R_t RR ps pt nths '(st_s, i_s) '(st_t, i_t),
-      (wsim_pre t υ ν E ∗ r R_s R_t RR ps pt nths (st_s, i_s) (st_t, i_t))%I.
+      (wsim_pre t υ ν E ∗ r R_s R_t RR ps pt nths (st_s, i_s) (st_t, i_t))%I. *)
 
-  (* Simulation relation that corresponds to iris' weakest precondition *)
-  Local Definition wsim_def
-      fl_s fl_t Ist (t : option bool) υ ν E r g R_s R_t RR ps pt nths st_s st_t
-      : iProp Σ :=
-    wsim_pre t υ ν E -∗
+  Local Definition wsim_def fl_s fl_t Ist Ep r g R_s R_t RR ps pt nths st_s st_t : iProp Σ :=
+    wsim_ginv Ep -∗
     @isim Σ open fl_s fl_t Ist r g R_s R_t RR ps pt nths st_s st_t.
   Local Definition wsim_aux : seal (@wsim_def). Proof using. by eexists. Qed.
   Definition wsim := wsim_aux.(unseal).
   Local Definition wsim_eq : @wsim = @wsim_def := wsim_aux.(seal_eq).
   Local Ltac unseal := rewrite wsim_eq /wsim_def.
 
-  Program Global Instance WP_refl
+  (* Program Global Instance WP_refl
       (υ : univ_id) (E : coPset)
     : WP (wsim_ginv υ E) υ E := mk_WP (wsim_ginv υ E) υ E True _.
   Next Obligation. ii; iSplit; first iIntros "$"; iIntros "[$ _]". Qed.
   
-  Program Global Instance wsim_fspec_precond (fsp : fspec) (υ : univ_id) m arg varg :
-    WP (precond (wsim_fspec υ fsp) m arg varg) υ ⊤ :=
-    mk_WP (precond (wsim_fspec υ fsp) m arg varg) υ ⊤ (precond fsp m arg varg) _.
+  Program Global Instance fspec_wsim_precond (fsp : fspec) (υ : univ_id) m arg varg :
+    WP (precond (fspec_wsim υ fsp) m arg varg) υ ⊤ :=
+    mk_WP (precond (fspec_wsim υ fsp) m arg varg) υ ⊤ (precond fsp m arg varg) _.
   Next Obligation. intros; iSplit; iIntros "[$ $]". Qed.
 
-  Program Global Instance wsim_fspec_postcond (fsp : fspec) (υ : univ_id) m arg varg :
-    WP (postcond (wsim_fspec υ fsp) m arg varg) υ ⊤ :=
+  Program Global Instance fspec_wsim_postcond (fsp : fspec) (υ : univ_id) m arg varg :
+    WP (postcond (fspec_wsim υ fsp) m arg varg) υ ⊤ :=
     {| WP_remainder := (postcond fsp m arg varg) |}.
-  Next Obligation. intros; iSplit; iIntros "[$ $]". Qed.
-
-  Lemma wsim_own_alloc `{!inG A Σ} (a : A) (VAL : ✓ a)
-    fl_s fl_t Ist b υ ν R_s R_t RR ps pt nths r g E st_s st_t i_s i_t :
-    ((∃ γ, own γ a) -∗ wsim fl_s fl_t Ist (Some b) υ ν E r g R_s R_t RR ps pt nths (st_s, i_s) (st_t, i_t))
-    ⊢ wsim fl_s fl_t Ist (Some b) υ ν E r g R_s R_t RR ps pt nths (st_s, i_s) (st_t, i_t).
-  Proof using.
-    destruct b; unseal; iIntros "SIM [O PRE]"; iMod (own_alloc a with "O") as "[O o]"; ss.
-    all: iApply ("SIM" with "o"); iFrame.
-  Qed.
-
-  Section lemmas.
+  Next Obligation. intros; iSplit; iIntros "[$ $]". Qed. *)
 
   Context (fl_s fl_t : alist string (Any.t → itree hmodE Any.t)).
   Context (Ist : nat → alist key Any.t → alist key Any.t → iProp Σ).
-
-  Local Notation wsim := (wsim fl_s fl_t Ist).
-
-  Context (t : option bool).
-  Context (υ ν : univ_id).
   Context (R_s R_t : Type).
+
+  Local Notation sim Ep r g := (wsim fl_s fl_t Ist Ep r g R_s R_t).
+  
+  Lemma wsim_own_alloc `{!inG A Σ} (a : A) Ew E r g RR ps pt nths st_s st_t i_s i_t :
+    ✓ a →
+    ((∃ γ, own γ a) -∗ sim (Some (Ew, E)) r g RR ps pt nths (st_s, i_s) (st_t, i_t))
+    ⊢ sim (Some (Ew, E)) r g RR ps pt nths (st_s, i_s) (st_t, i_t).
+  Proof using.
+    unseal; iIntros (?) "SIM [O PRE]"; iMod (own_alloc a with "O") as "[O o]"; ss.
+    iApply ("SIM" with "o"); iFrame.
+  Qed.
+
+  Context (Ep : option (coPset * coPset)).
+  Context (r g : rel).
   Context (RR : post R_s R_t).
   Context (ps pt : bool).
   Context (nths : nat).
   Context (st_s st_t : state).
 
-  Lemma wsim_ret r g rs rt :
+  Lemma wsim_ret rs rt :
     RR nths (st_s, rs) (st_t, rt) ⊢
-    wsim t υ ν ⊤ r g R_s R_t RR ps pt nths (st_s, Ret rs) (st_t, Ret rt).
-  Proof using. unseal; iIntros "RR I". iApply isim_ret. iFrame. Qed.
+    sim Ep r g RR ps pt nths (st_s, Ret rs) (st_t, Ret rt).
+  Proof using. unseal; iIntros "RR I". by iApply isim_ret. Qed.
 
-  Lemma wsim_call r g E k_s k_t fn arg :
+  Lemma wsim_call fn arg k_s k_t :
     Ist nths st_s st_t ∗
     (∀ ret nths' st_s' st_t'
       (NODS : List.NoDup (List.map fst st_s'))
       (NODD : List.NoDup (List.map fst st_t')),
       Ist nths' st_s' st_t' -∗
-      wsim t υ ν E r g R_s R_t RR true true nths' (st_s', k_s ret) (st_t', k_t ret)) ⊢
-    wsim t υ ν E r g R_s R_t RR ps pt nths
+      sim Ep r g RR true true nths' (st_s', k_s ret) (st_t', k_t ret)) ⊢
+    sim Ep r g RR ps pt nths
       (st_s, trigger (Call fn arg) >>= k_s) (st_t, trigger (Call fn arg) >>= k_t).
   Proof using.
     unseal; iIntros "[IST CONT] I".
@@ -140,248 +138,209 @@ Section wsim.
     iIntros (??????) "IST"; iApply ("CONT" with "[] [] [IST]"); iFrame; try iPureIntro; ss.
   Qed.
 
-  Lemma wsim_call_sandbox r g E k_s k_t fn arg (mask_src mask_tgt:_→bool) scopes_src scopes_tgt:
+  Lemma wsim_call_sandbox fn arg k_s k_t (mask_src mask_tgt : _ → bool) scopes_src scopes_tgt :
     (mask_src fn) → (mask_tgt fn) →
     Ist nths st_s st_t ∗
     (∀ ret nths' st_s' st_t'
       (NODS : List.NoDup (List.map fst st_s'))
       (NODD : List.NoDup (List.map fst st_t')),
       Ist nths' st_s' st_t' -∗
-      wsim t υ ν E r g R_s R_t RR true true nths' (st_s', k_s ret) (st_t', k_t ret)) ⊢
-    wsim t υ ν E r g R_s R_t RR ps pt nths
-      (st_s, HModTr.sandbox mask_src scopes_src (trigger (Call fn arg)) >>= k_s) (st_t, HModTr.sandbox mask_tgt scopes_tgt (trigger (Call fn arg)) >>= k_t).
+      sim Ep r g RR true true nths' (st_s', k_s ret) (st_t', k_t ret)) ⊢
+    sim Ep r g RR ps pt nths
+      (st_s, HModTr.sandbox mask_src scopes_src (trigger (Call fn arg)) >>= k_s)
+      (st_t, HModTr.sandbox mask_tgt scopes_tgt (trigger (Call fn arg)) >>= k_t).
   Proof using.
-  i. iIntros "ISIM".
-  rewrite !SBRed.call.
-  des_ifs; ss.
-  iApply wsim_call. iFrame.
+    iIntros (??) "SIM"; rewrite !SBRed.call; des_ifs; ss; iApply wsim_call; done.
   Qed.
   
-  Lemma wsim_io r g fn I O (arg : I) k_s k_t E :
+  Lemma wsim_io fn I O (arg : I) k_s k_t :
     (∀ (ret : O),
-      wsim t υ ν E r g R_s R_t RR true true nths (st_s, k_s ret) (st_t, k_t ret)) ⊢
-    wsim t υ ν E r g R_s R_t RR ps pt nths
+      sim Ep r g RR true true nths (st_s, k_s ret) (st_t, k_t ret)) ⊢
+    sim Ep r g RR ps pt nths
       (st_s, trigger (IO fn arg) >>= k_s)
       (st_t, trigger (IO fn arg) >>= k_t).
   Proof using. unseal; iIntros "RR I". iApply isim_io. iIntros (ret); iApply "RR"; iFrame. Qed.
 
-  Lemma wsim_tau_src r g i_s i_t E :
-    wsim t υ ν E r g R_s R_t RR true pt nths (st_s, i_s) (st_t, i_t) ⊢
-    wsim t υ ν E r g R_s R_t RR ps pt nths (st_s, tau;; i_s) (st_t, i_t).
+  Lemma wsim_tau_src i_s i_t :
+    sim Ep r g RR true pt nths (st_s, i_s) (st_t, i_t) ⊢
+    sim Ep r g RR ps pt nths (st_s, tau;; i_s) (st_t, i_t).
   Proof using. unseal; iIntros "RR I". iApply isim_tau_src; iApply "RR"; iFrame. Qed.
 
-  Lemma wsim_tau_tgt r g i_s i_t E :
-    wsim t υ ν E r g R_s R_t RR ps true nths (st_s, i_s) (st_t, i_t) ⊢
-    wsim t υ ν E r g R_s R_t RR ps pt nths (st_s, i_s) (st_t, tau;; i_t).
+  Lemma wsim_tau_tgt i_s i_t :
+    sim Ep r g RR ps true nths (st_s, i_s) (st_t, i_t) ⊢
+    sim Ep r g RR ps pt nths (st_s, i_s) (st_t, tau;; i_t).
   Proof using. unseal; iIntros "RR I". iApply isim_tau_tgt; iApply "RR"; iFrame. Qed.
 
-  Lemma wsim_inline_src r g fn arg f_s k_s i_t E :
+  Lemma wsim_inline_src fn arg f_s k_s i_t :
     alist_find fn fl_s = Some f_s →
-    wsim t υ ν E r g R_s R_t RR true pt nths
+    sim Ep r g RR true pt nths
       (st_s, x <- (ret <- (f_s arg);; (tau;; Ret ret));; (k_s x))
       (st_t, i_t) ⊢
-    wsim t υ ν E r g R_s R_t RR ps pt nths (st_s, trigger (Call fn arg) >>= k_s) (st_t, i_t).
+    sim Ep r g RR ps pt nths (st_s, trigger (Call fn arg) >>= k_s) (st_t, i_t).
   Proof using. i; unseal; iIntros "RR I". iApply isim_inline_src; eauto. iApply "RR"; iFrame. Qed.
 
-  Lemma wsim_inline_src_sandbox r g fn arg f_s k_s i_t E (mask:_→bool) scopes:
+  Lemma wsim_inline_src_sandbox fn arg f_s k_s i_t (mask : _ → bool) scopes :
     alist_find fn fl_s = Some f_s →
-    (mask fn) →
-    wsim t υ ν E r g R_s R_t RR true pt nths
+    mask fn →
+    sim Ep r g RR true pt nths
       (st_s, x <- (ret <- (f_s arg);; (tau;; Ret ret));; (k_s x))
       (st_t, i_t) ⊢
-    wsim t υ ν E r g R_s R_t RR ps pt nths (st_s, HModTr.sandbox mask scopes (trigger (Call fn arg)) >>= k_s) (st_t, i_t).
+    sim Ep r g RR ps pt nths
+      (st_s, HModTr.sandbox mask scopes (trigger (Call fn arg)) >>= k_s)
+      (st_t, i_t).
   Proof using.
-    i. iIntros "ISIM".
-    rewrite SBRed.call.
-    des_ifs; ss.
-    iApply wsim_inline_src; eauto.
+    i. iIntros "ISIM". rewrite SBRed.call. des_ifs; ss. iApply wsim_inline_src; eauto.
   Qed.
 
-  Lemma wsim_inline_tgt r g fn arg i_s f_t k_t E :
+  Lemma wsim_inline_tgt fn arg f_t i_s k_t :
     alist_find fn fl_t = Some f_t →
-    wsim t υ ν E r g R_s R_t RR ps true nths
+    sim Ep r g RR ps true nths
       (st_s, i_s)
       (st_t, x <- (ret <- (f_t arg);; (tau;; Ret ret));; (k_t x)) ⊢
-    wsim t υ ν E r g R_s R_t RR ps pt nths (st_s, i_s) (st_t, trigger (Call fn arg) >>= k_t).
+    sim Ep r g RR ps pt nths (st_s, i_s) (st_t, trigger (Call fn arg) >>= k_t).
   Proof using. i; unseal; iIntros "RR I". iApply isim_inline_tgt; eauto. iApply "RR"; iFrame. Qed.
 
-  Lemma wsim_inline_tgt_sandbox r g fn arg i_s f_t k_t E (mask:_→bool) scopes:
+  Lemma wsim_inline_tgt_sandbox fn arg f_t i_s k_t (mask : _ → bool) scopes :
     alist_find fn fl_t = Some f_t →
-    (mask fn) →
-    wsim t υ ν E r g R_s R_t RR ps true nths
+    mask fn →
+    sim Ep r g RR ps true nths
       (st_s, i_s)
       (st_t, x <- (ret <- (f_t arg);; (tau;; Ret ret));; (k_t x)) ⊢
-    wsim t υ ν E r g R_s R_t RR ps pt nths (st_s, i_s) (st_t, HModTr.sandbox mask scopes (trigger (Call fn arg)) >>= k_t).
+    sim Ep r g RR ps pt nths
+      (st_s, i_s)
+      (st_t, HModTr.sandbox mask scopes (trigger (Call fn arg)) >>= k_t).
   Proof using.
-  i. iIntros "ISIM".
-  rewrite SBRed.call.
-  des_ifs; ss.
-  iApply wsim_inline_tgt; eauto.
+    i. iIntros "ISIM". rewrite SBRed.call. des_ifs; ss. iApply wsim_inline_tgt; eauto.
   Qed.
   
-  Lemma wsim_take_src X r g k_s i_t E :
-    (∀ x, wsim t υ ν E r g R_s R_t RR true pt nths
-      (st_s, k_s x) (st_t, i_t)) ⊢
-    wsim t υ ν E r g R_s R_t RR ps pt nths
-      (st_s, trigger (Take X) >>= k_s) (st_t, i_t).
+  Lemma wsim_take_src X k_s i_t :
+    (∀ x, sim Ep r g RR true pt nths (st_s, k_s x) (st_t, i_t)) ⊢
+    sim Ep r g RR ps pt nths (st_s, trigger (Take X) >>= k_s) (st_t, i_t).
   Proof using.
     unseal; iIntros "RR I". iApply isim_take_src; eauto. iIntros (x); iApply "RR"; iFrame.
   Qed.
 
-  Lemma wsim_take_tgt X r g i_s k_t E :
-    (∃ x,
-      wsim t υ ν E r g R_s R_t RR ps true nths (st_s, i_s) (st_t, k_t x)) ⊢
-    wsim t υ ν E r g R_s R_t RR ps pt nths
-      (st_s, i_s) (st_t, trigger (Take X) >>= k_t).
+  Lemma wsim_take_tgt X i_s k_t :
+    (∃ x, sim Ep r g RR ps true nths (st_s, i_s) (st_t, k_t x)) ⊢
+    sim Ep r g RR ps pt nths (st_s, i_s) (st_t, trigger (Take X) >>= k_t).
   Proof using.
     unseal; iIntros "[%x RR] I". iApply isim_take_tgt; eauto. iExists _; iApply "RR"; iFrame.
   Qed.
 
-  Lemma wsim_choose_src X r g k_s i_t E :
-    (∃ x,
-      wsim t υ ν E r g R_s R_t RR true pt nths (st_s, k_s x) (st_t, i_t)) ⊢
-    wsim t υ ν E r g R_s R_t RR ps pt nths
-      (st_s, trigger (Choose X) >>= k_s) (st_t, i_t).
+  Lemma wsim_choose_src X k_s i_t :
+    (∃ x, sim Ep r g RR true pt nths (st_s, k_s x) (st_t, i_t)) ⊢
+    sim Ep r g RR ps pt nths (st_s, trigger (Choose X) >>= k_s) (st_t, i_t).
   Proof using.
     unseal; iIntros "[%x RR] I". iApply isim_choose_src; eauto. iExists _; iApply "RR"; iFrame.
   Qed.
 
-  Lemma wsim_choose_tgt X r g i_s k_t E :
-    (∀ x,
-      wsim t υ ν E r g R_s R_t RR ps true nths (st_s, i_s) (st_t, k_t x)) ⊢
-    wsim t υ ν E r g R_s R_t RR ps pt nths
-      (st_s, i_s) (st_t, trigger (Choose X) >>= k_t).
+  Lemma wsim_choose_tgt X i_s k_t :
+    (∀ x, sim Ep r g RR ps true nths (st_s, i_s) (st_t, k_t x)) ⊢
+    sim Ep r g RR ps pt nths (st_s, i_s) (st_t, trigger (Choose X) >>= k_t).
   Proof using.
     unseal; iIntros "RR I". iApply isim_choose_tgt; eauto. iIntros (x); iApply "RR"; iFrame.
   Qed.
 
-  Lemma wsim_sput_src k v r g k_s i_t E :
-    wsim t υ ν E r g R_s R_t RR true pt nths
-      (alist_upd k v st_s, k_s tt) (st_t, i_t) ⊢
-    wsim t υ ν E r g R_s R_t RR ps pt nths
-      (st_s, trigger (SPut k v) >>= k_s) (st_t, i_t).
+  Lemma wsim_sput_src k v k_s i_t :
+    sim Ep r g RR true pt nths (alist_upd k v st_s, k_s tt) (st_t, i_t) ⊢
+    sim Ep r g RR ps pt nths (st_s, trigger (SPut k v) >>= k_s) (st_t, i_t).
   Proof using. unseal; iIntros "RR I". iApply isim_sput_src; eauto. iApply "RR"; iFrame. Qed.
 
-  Lemma wsim_sput_tgt k v r g i_s k_t E :
-    wsim t υ ν E r g R_s R_t RR ps true nths
-      (st_s, i_s) (alist_upd k v st_t, k_t tt) ⊢
-    wsim t υ ν E r g R_s R_t RR ps pt nths
-      (st_s, i_s) (st_t, trigger (SPut k v) >>= k_t).
+  Lemma wsim_sput_tgt k v i_s k_t :
+    sim Ep r g RR ps true nths (st_s, i_s) (alist_upd k v st_t, k_t tt) ⊢
+    sim Ep r g RR ps pt nths (st_s, i_s) (st_t, trigger (SPut k v) >>= k_t).
   Proof using. unseal; iIntros "RR I". iApply isim_sput_tgt; eauto. iApply "RR"; iFrame. Qed.
 
-  Lemma wsim_sget_src k r g k_s i_t E :
-    wsim t υ ν E r g R_s R_t RR true pt nths
-      (st_s, k_s (or_else (alist_find k st_s) tt↑)) (st_t, i_t) ⊢
-    wsim t υ ν E r g R_s R_t RR ps pt nths
-      (st_s, trigger (SGet k) >>= k_s) (st_t, i_t).
+  Lemma wsim_sget_src k k_s i_t :
+    sim Ep r g RR true pt nths (st_s, k_s (or_else (alist_find k st_s) tt↑)) (st_t, i_t) ⊢
+    sim Ep r g RR ps pt nths (st_s, trigger (SGet k) >>= k_s) (st_t, i_t).
   Proof using. unseal; iIntros "RR I". iApply isim_sget_src; eauto. iApply "RR"; iFrame. Qed.
 
-  Lemma wsim_sget_tgt k r g i_s k_t E :
-    wsim t υ ν E r g R_s R_t RR ps true nths
-      (st_s, i_s) (st_t, k_t (or_else (alist_find k st_t) tt↑)) ⊢
-    wsim t υ ν E r g R_s R_t RR ps pt nths
-      (st_s, i_s) (st_t, trigger (SGet k) >>= k_t).
+  Lemma wsim_sget_tgt k i_s k_t :
+    sim Ep r g RR ps true nths (st_s, i_s) (st_t, k_t (or_else (alist_find k st_t) tt↑)) ⊢
+    sim Ep r g RR ps pt nths (st_s, i_s) (st_t, trigger (SGet k) >>= k_t).
   Proof using. unseal; iIntros "RR I". iApply isim_sget_tgt; eauto. iApply "RR"; iFrame. Qed.
 
-  Lemma wsim_assume_src P r g k_s i_t E :
-    (P -∗ wsim t υ ν E r g R_s R_t RR true pt nths
-      (st_s, k_s tt) (st_t, i_t)) ⊢
-    wsim t υ ν E r g R_s R_t RR ps pt nths
-      (st_s, trigger (Assume P) >>= k_s) (st_t, i_t).
+  Lemma wsim_assume_src P k_s i_t :
+    (P -∗ sim Ep r g RR true pt nths (st_s, k_s tt) (st_t, i_t)) ⊢
+    sim Ep r g RR ps pt nths (st_s, trigger (Assume P) >>= k_s) (st_t, i_t).
   Proof using.
     unseal; iIntros "RR I". iApply isim_assume_src; eauto. iIntros "P".
     iApply ("RR" with "P"); iFrame.
   Qed.
 
-  Lemma wsim_assume_precise_src P r g k_s i_t E
-    :
-    precise P
-    ∗
-    (P -∗ wsim t υ ν E r g R_s R_t RR true pt nths
-      (st_s, k_s tt) (st_t, i_t)) ⊢
-    wsim t υ ν E r g R_s R_t RR ps pt nths
-      (st_s, trigger (AssumePrecise P) >>= k_s) (st_t, i_t).
+  Lemma wsim_assume_precise_src P k_s i_t :
+    precise P ∗
+    (P -∗ sim Ep r g RR true pt nths (st_s, k_s tt) (st_t, i_t)) ⊢
+    sim Ep r g RR ps pt nths (st_s, trigger (AssumePrecise P) >>= k_s) (st_t, i_t).
   Proof using.
     unseal. iIntros "[P H] I". iApply isim_assume_precise_src; eauto.
     iFrame. iIntros "P". iApply ("H" with "P I").
   Qed.
 
-  Lemma wsim_assume_tgt P r g i_s k_t E :
-    P ∗ wsim t υ ν E r g R_s R_t RR ps true nths
-      (st_s, i_s) (st_t, k_t tt) ⊢
-    wsim t υ ν E r g R_s R_t RR ps pt nths
-      (st_s, i_s) (st_t, trigger (Assume P) >>= k_t).
-  Proof using. unseal; iIntros "[P RR] I". iApply isim_assume_tgt; eauto. iFrame. iApply "RR". ss. Qed.
+  Lemma wsim_assume_tgt P i_s k_t :
+    P ∗ sim Ep r g RR ps true nths (st_s, i_s) (st_t, k_t tt) ⊢
+    sim Ep r g RR ps pt nths (st_s, i_s) (st_t, trigger (Assume P) >>= k_t).
+  Proof using.
+    unseal; iIntros "[P RR] I". iApply isim_assume_tgt; eauto. iFrame. iApply "RR". ss.
+  Qed.
 
-  Lemma wsim_assume_precise_tgt P r g i_s k_t E :
-    (precise P -∗ P ∗ wsim t υ ν E r g R_s R_t RR ps true nths
-          (st_s, i_s) (st_t, k_t tt)) ⊢
-    wsim t υ ν E r g R_s R_t RR ps pt nths
-      (st_s, i_s) (st_t, trigger (AssumePrecise P) >>= k_t).
+  Lemma wsim_assume_precise_tgt P i_s k_t :
+    (precise P -∗ P ∗ sim Ep r g RR ps true nths (st_s, i_s) (st_t, k_t tt)) ⊢
+    sim Ep r g RR ps pt nths (st_s, i_s) (st_t, trigger (AssumePrecise P) >>= k_t).
   Proof using.
     unseal; iIntros "H I". iApply isim_assume_precise_tgt; eauto.
-    iIntros "P". iPoseProof ("H" with "P") as "[P H]".
-    iFrame. iApply "H". et.
+    iIntros "P". iPoseProof ("H" with "P") as "[P H]". iFrame. iApply "H". done.
   Qed.
 
-  Lemma wsim_assume_precise_both P r g k_s k_t E :
-    (wsim t υ ν E r g R_s R_t RR true true nths
-      (st_s, k_s tt) (st_t, k_t tt))
-    ⊢ wsim t υ ν E r g R_s R_t RR ps pt nths
-      (st_s, trigger (AssumePrecise P) >>= k_s) (st_t, trigger (AssumePrecise P) >>= k_t).
+  Lemma wsim_assume_precise_both P k_s k_t :
+    (sim Ep r g RR true true nths (st_s, k_s tt) (st_t, k_t tt)) ⊢
+    sim Ep r g RR ps pt nths
+      (st_s, trigger (AssumePrecise P) >>= k_s)
+      (st_t, trigger (AssumePrecise P) >>= k_t).
   Proof using.
-    unseal. iIntros "RR I". iApply isim_assume_precise_both; eauto.
-    iApply "RR". et.
+    unseal. iIntros "RR I". iApply isim_assume_precise_both; eauto. by iApply "RR".
   Qed.
 
-  Lemma wsim_guarantee_src (P : iProp Σ) r g k_s i_t E :
-    P ∗ wsim t υ ν E r g R_s R_t RR true pt nths
-      (st_s, k_s tt) (st_t, i_t) ⊢
-    wsim t υ ν E r g R_s R_t RR ps pt nths
-      (st_s, trigger (Guarantee P) >>= k_s) (st_t, i_t).
+  Lemma wsim_guarantee_src (P : iProp Σ) k_s i_t :
+    P ∗ sim Ep r g RR true pt nths (st_s, k_s tt) (st_t, i_t) ⊢
+    sim Ep r g RR ps pt nths (st_s, trigger (Guarantee P) >>= k_s) (st_t, i_t).
   Proof using.
     unseal; iIntros "[P RR] I". iApply isim_guarantee_src; eauto. iFrame. iApply "RR"; ss.
   Qed.
 
-  Lemma wsim_guarantee_tgt (P : iProp Σ) r g i_s k_t E :
-    (P -∗ wsim t υ ν E r g R_s R_t RR ps true nths
-      (st_s, i_s) (st_t, k_t tt)) ⊢
-    wsim t υ ν E r g R_s R_t RR ps pt nths
-      (st_s, i_s) (st_t, trigger (Guarantee P) >>= k_t).
+  Lemma wsim_guarantee_tgt (P : iProp Σ) i_s k_t :
+    (P -∗ sim Ep r g RR ps true nths (st_s, i_s) (st_t, k_t tt)) ⊢
+    sim Ep r g RR ps pt nths (st_s, i_s) (st_t, trigger (Guarantee P) >>= k_t).
   Proof using.
     unseal; iIntros "RR I". iApply isim_guarantee_tgt; eauto.
     iIntros "P"; iApply ("RR" with "P"); done.
   Qed.
 
-  Lemma wsim_spawn r g fn args k_s k_t E :
-    wsim t υ ν E r g R_s R_t RR true true (S nths)
-      (st_s, k_s nths) (st_t, k_t nths) ⊢
-    wsim t υ ν E r g R_s R_t RR ps pt nths
+  Lemma wsim_spawn fn args k_s k_t :
+    sim Ep r g RR true true (S nths) (st_s, k_s nths) (st_t, k_t nths) ⊢
+    sim Ep r g RR ps pt nths
       (st_s, trigger (Spawn fn args) >>= k_s)
       (st_t, trigger (Spawn fn args) >>= k_t).
   Proof using. unseal; iIntros "C I". iApply isim_spawn; eauto. iApply "C". ss. Qed.
 
-  Lemma wsim_spawn_sandbox r g fn args k_s k_t E (mask_src mask_tgt:_→bool) scopes_src scopes_tgt:
-    (mask_src fn) → (mask_tgt fn) →
-    wsim t υ ν E r g R_s R_t RR true true (S nths)
-      (st_s, k_s nths) (st_t, k_t nths) ⊢
-    wsim t υ ν E r g R_s R_t RR ps pt nths
+  Lemma wsim_spawn_sandbox fn args k_s k_t (mask_src mask_tgt : _ → bool) scopes_src scopes_tgt :
+    mask_src fn → mask_tgt fn →
+    sim Ep r g RR true true (S nths) (st_s, k_s nths) (st_t, k_t nths) ⊢
+    sim Ep r g RR ps pt nths
       (st_s, HModTr.sandbox mask_src scopes_src (trigger (Spawn fn args)) >>= k_s)
       (st_t, HModTr.sandbox mask_tgt scopes_tgt (trigger (Spawn fn args)) >>= k_t).
   Proof using.
-  i. iIntros "ISIM".
-  rewrite !SBRed.spawn.
-  des_ifs; ss.
-  iApply wsim_spawn. iFrame.
+    i. iIntros "ISIM". rewrite !SBRed.spawn. des_ifs; ss. iApply wsim_spawn. iFrame.
   Qed.
   
-  Lemma wsim_yield r g tid k_s k_t E :
+  Lemma wsim_yield tid k_s k_t :
     Ist nths st_s st_t ∗
     (∀ nths' st_s' st_t' (NODS : List.NoDup (map fst st_s')) (NODT : List.NoDup (map fst st_t')),
       Ist nths' st_s' st_t' -∗
-      wsim t υ ν E r g R_s R_t RR true true nths'
+      sim Ep r g RR true true nths'
         (st_s', k_s tt) (st_t', k_t tt)) ⊢
-    wsim t υ ν E r g R_s R_t RR ps pt nths
+    sim Ep r g RR ps pt nths
       (st_s, trigger (Yield tid) >>= k_s)
       (st_t, trigger (Yield tid) >>= k_t).
   Proof using.
@@ -389,39 +348,39 @@ Section wsim.
     iIntros (?????) "IST"; iApply ("C" with "[] [] [IST] [I]"); iFrame; iPureIntro; ss.
   Qed.
 
-  Lemma wsim_reset r g i_s i_t E :
-    wsim t υ ν E r g R_s R_t RR false false nths (st_s, i_s) (st_t, i_t) ⊢
-    wsim t υ ν E r g R_s R_t RR ps pt nths (st_s, i_s) (st_t, i_t).
+  Lemma wsim_reset i_s i_t :
+    sim Ep r g RR false false nths (st_s, i_s) (st_t, i_t) ⊢
+    sim Ep r g RR ps pt nths (st_s, i_s) (st_t, i_t).
   Proof using. unseal; iIntros "RR I". iApply isim_reset; iApply "RR"; iFrame. Qed.
 
-  Lemma wsim_progress r g i_s i_t E :
-    wsim t υ ν E g g R_s R_t RR false false nths (st_s, i_s) (st_t, i_t) ⊢
-    wsim t υ ν E r g R_s R_t RR true true nths (st_s, i_s) (st_t, i_t).
+  Lemma wsim_progress i_s i_t :
+    sim Ep g g RR false false nths (st_s, i_s) (st_t, i_t) ⊢
+    sim Ep r g RR true true nths (st_s, i_s) (st_t, i_t).
   Proof using. unseal; iIntros "RR I". iApply isim_progress; iApply "RR"; iFrame. Qed.
 
   (* Lemma wsim_base r g i_s i_t :
-    r R_s R_t RR ps pt nths (st_s, i_s) (st_t, i_t) ⊢
-    wsim t υ ν ⊤ r g R_s R_t RR ps pt nths
+    r RR ps pt nths (st_s, i_s) (st_t, i_t) ⊢
+    sim ⊤ r g RR ps pt nths
       (st_s, i_s) (st_t, i_t).
   Proof using. unseal; iIntros "RR I". iApply isim_base; iFrame. Qed. *)
 
-  Lemma wsim_base_t r g i_s i_t :
-    (wsim_pre t υ ν ⊤ -∗ r R_s R_t RR ps pt nths (st_s, i_s) (st_t, i_t)) ⊢
-    wsim t υ ν ⊤ r g R_s R_t RR ps pt nths
-      (st_s, i_s) (st_t, i_t).
+  Lemma wsim_base_t i_s i_t :
+    (wsim_ginv Ep -∗ r R_s R_t RR ps pt nths (st_s, i_s) (st_t, i_t)) ⊢
+    sim Ep r g RR ps pt nths (st_s, i_s) (st_t, i_t).
   Proof using. unseal; iIntros "RR I". iApply isim_base; iRevert "I"; iFrame. Qed.
 
-  Lemma wsim_coind (r g : rel) A P RA_s RA_t RRA psA ptA nthsA srcA tgtA :
+  Lemma wsim_coind A P RA_s RA_t RRA psA ptA nthsA srcA tgtA :
     (∀ (g' : rel) (a : A),
       P a -∗
-      (⌜∀ R_s R_t RR ps pt nths0 src tgt,
+      (⌜∀ RR ps pt nths0 src tgt,
         g R_s R_t RR ps pt nths0 src tgt -∗ g' R_s R_t RR ps pt nths0 src tgt⌝) -∗
-      (□ ∀ a, (P a ∗ wsim_pre t υ ν ⊤) -∗
+      (□ ∀ a, (P a ∗ wsim_ginv Ep) -∗
         g' (RA_s a) (RA_t a) (RRA a) (psA a) (ptA a) (nthsA a) (srcA a) (tgtA a)) -∗
-      wsim t υ ν ⊤ r g'
+      wsim fl_s fl_t Ist Ep r g'
         (RA_s a) (RA_t a) (RRA a) (psA a) (ptA a) (nthsA a) (srcA a) (tgtA a)) →
     ∀ (a : A), P a ⊢
-      wsim t υ ν ⊤ r g (RA_s a) (RA_t a) (RRA a) (psA a) (ptA a) (nthsA a) (srcA a) (tgtA a).
+      wsim fl_s fl_t Ist Ep r g
+        (RA_s a) (RA_t a) (RRA a) (psA a) (ptA a) (nthsA a) (srcA a) (tgtA a).
   Proof using.
     unseal; intros H a; iIntros "P I"; iCombine "P I" as "P". iStopProof.
     (* rewrite /wsim_retcond *)
@@ -429,7 +388,7 @@ Section wsim.
     intros g' a Himpl; iIntros "[[P I] #CIH]".
     iPoseProof (H with "P [] [] I") as "H".
     { instantiate (1 := g').
-      iPureIntro; iIntros (????????) "G"; destruct src, tgt. iApply Himpl. iFrame.
+      iPureIntro; iIntros (??????) "G"; destruct src, tgt. iApply Himpl. iFrame.
     }
     { iModIntro; iIntros (a') "[P I]"; iSpecialize ("CIH" $! a'); destruct (srcA a'), (tgtA a').
       iApply "CIH"; iFrame.
@@ -439,111 +398,117 @@ Section wsim.
     { iIntros (????????) "H !>"; destruct sti_src, sti_tgt; iFrame. }
   Qed.
 
-  Lemma wsim_bind r g {Qs Qt} QQ i_s i_t k_s k_t E :
-    wsim t υ ν E r g Qs Qt QQ ps pt nths (st_s, i_s) (st_t, i_t)
+  Lemma wsim_bind {Qs Qt} QQ i_s i_t k_s k_t :
+    wsim fl_s fl_t Ist Ep r g Qs Qt QQ ps pt nths (st_s, i_s) (st_t, i_t)
     ∗ (∀ nths st_s' r_s st_t' r_t,
         QQ nths (st_s', r_s) (st_t', r_t)
-        -∗ wsim None υ ν E r g R_s R_t RR false false nths (st_s', k_s r_s) (st_t', k_t r_t))%I
-    ⊢ (wsim t υ ν E r g R_s R_t RR ps pt nths (st_s, i_s >>= k_s) (st_t, i_t >>= k_t)).
+        -∗ sim None r g RR false false nths (st_s', k_s r_s) (st_t', k_t r_t))%I
+    ⊢ sim Ep r g RR ps pt nths (st_s, i_s >>= k_s) (st_t, i_t >>= k_t).
   Proof using.
-    rewrite wsim.wsim_eq /wsim.wsim_def /wsim.wsim_pre.
+    rewrite wsim.wsim_eq /wsim.wsim_def.
     iIntros "[W SIM] INV". iApply isim_bind.
     iSplitL "W INV". { iApply "W"; eauto. }
     iIntros (? ? ? ? ?) "Q". iApply ("SIM" with "Q"). done.
   Qed.
 
   (* ginv related lemmas *)
-  Lemma wsim_full_guarantee_src_WP `{i : !WP P υ E} r g k_s i_t :
+  Lemma wsim_guarantee_src_WP `{i : !WP P Ew' E'} k_s i_t Ew E :
+    Ew' ⊆ Ew → E' ⊆ E →
     (WP_remainder i ∗
-    wsim None υ ν E r g R_s R_t RR true pt nths (st_s, k_s tt) (st_t, i_t)) ⊢
-    wsim (Some true) υ ν E r g R_s R_t RR ps pt nths
-      (st_s, trigger (Guarantee P) >>= k_s) (st_t, i_t).
+    sim (Some (Ew ∖ Ew', E ∖ E')) r g RR true pt nths (st_s, k_s tt) (st_t, i_t)) ⊢
+    sim (Some (Ew, E)) r g RR ps pt nths (st_s, trigger (Guarantee P) >>= k_s) (st_t, i_t).
   Proof using.
-    unseal; iIntros "[P SIM] I". iApply isim_guarantee_src; eauto.
-    iSplitR "SIM".
-    { iApply WP_iff; iFrame. }
-    { iApply "SIM"; done. }
-  Qed.
-
-  Lemma wsim_full_guarantee_src_upd (P : iProp Σ) r g k_s i_t E :
-    ((wsim_ginv υ E ==∗ P) ∗
-    wsim None υ ν E r g R_s R_t RR true pt nths
-      (st_s, k_s tt) (st_t, i_t)) ⊢
-    wsim (Some true) υ ν E r g R_s R_t RR ps pt nths
-      (st_s, trigger (Guarantee P) >>= k_s) (st_t, i_t).
-  Proof using.
-    unseal; iIntros "[P SIM] I".
-    iPoseProof ("P" with "I") as ">P".
+    unseal; iIntros (??) "[P SIM] [O [E [%n W]]]".
+    iMod (own_admin_split with "O") as "[O1 O2]".
     iApply isim_guarantee_src; eauto.
-    iSplitR "SIM"; iFrame. iApply "SIM"; done.
+    rewrite /wsim_ginv {2}(union_difference_L Ew' Ew) // wsats_split; last set_solver.
+    rewrite {2}(union_difference_L E' E) // ownE_op; last set_solver.
+    iDestruct "W" as "[W1 W2]"; iDestruct "E" as "[E1 E2]".
+    iSplitR "E2 W2 O2 SIM".
+    { iApply WP_iff; iFrame. }
+    { iApply "SIM"; iFrame. }
   Qed.
 
-  Lemma wsim_full_guarantee_src (P : iProp Σ) r g k_s i_t E :
+  (* Lemma wsim_full_guarantee_src (P : iProp Σ) k_s i_t Ew E :
+    ((wsim_ginv (Some (Ew, E)) ==∗ P) ∗ sim None r g RR true pt nths (st_s, k_s tt) (st_t, i_t)) ⊢
+    sim (Some (Ew, E)) r g RR ps pt nths (st_s, trigger (Guarantee P) >>= k_s) (st_t, i_t).
+  Proof using.
+    unseal; iIntros "[P SIM] I". iPoseProof ("P" with "I") as ">P".
+    iApply isim_guarantee_src; eauto. iSplitR "SIM"; iFrame. iApply "SIM"; done.
+  Qed. *)
+
+  (* Lemma wsim_full_guarantee_src (P : iProp Σ) r g k_s i_t E :
     ((wsim_ginv υ E -∗ P) ∗
-    wsim None υ ν E r g R_s R_t RR true pt nths
-      (st_s, k_s tt) (st_t, i_t)) ⊢
-    wsim (Some true) υ ν E r g R_s R_t RR ps pt nths
-      (st_s, trigger (Guarantee P) >>= k_s) (st_t, i_t).
+    wsim None υ ν E r g RR true pt nths (st_s, k_s tt) (st_t, i_t)) ⊢
+    wsim (Some true) υ ν E r g RR ps pt nths (st_s, trigger (Guarantee P) >>= k_s) (st_t, i_t).
   Proof using.
     unseal; iIntros "[P SIM] I". iApply isim_guarantee_src; eauto.
     iSplitR "SIM"; iFrame. iApply "P"; iFrame. iApply "SIM"; done.
-  Qed.
+  Qed. *)
 
-  Lemma wsim_full_assume_src_WP `{i : !WP P υ E} r g k_s i_t :
-    (WP_remainder i -∗ wsim (Some true) υ ν E r g R_s R_t RR true pt nths
-      (st_s, k_s tt) (st_t, i_t)) ⊢
-    wsim None υ ν E r g R_s R_t RR ps pt nths
-      (st_s, trigger (Assume P) >>= k_s) (st_t, i_t).
+  (* let Ep' := match Ep with | Some (Ew, Ee) => Some (Ew ∪ E, Ee ∪ E) | None => Some (E, E) end in *)
+  Lemma wsim_assume_src_WP `{i : !WP P Ew' E'} k_s i_t :
+    let Ep' :=
+      match Ep with | Some (Ew, E) => Some (Ew ∪ Ew', E ∪ E') | None => Some (Ew', E') end
+    in
+    (WP_remainder i -∗ sim Ep' r g RR true pt nths (st_s, k_s tt) (st_t, i_t)) ⊢
+    sim Ep r g RR ps pt nths (st_s, trigger (Assume P) >>= k_s) (st_t, i_t).
   Proof using.
-    unseal; iIntros "SIM _". iApply isim_assume_src; eauto.
-    iIntros "P". iPoseProof (WP_iff with "P") as "[I Q]".
-    iApply ("SIM" with "Q I").
+    unseal; iIntros "SIM I1". iApply isim_assume_src; eauto. iIntros "P".
+    destruct Ep as [[??]|]; iPoseProof (WP_iff with "P") as "[I Q]";
+      try iApply ("SIM" with "Q I").
+    rewrite /wsim_ginv; iPoseProof ("SIM" with "Q") as "SIM".
+    iDestruct "I1" as "[O [E [%n1 W]]]". iDestruct "I" as "[_ [E2 [%n2 W2]]]".
+    iPoseProof (ownE_exploit with "[E E2]") as "%"; first iFrame.
+    iMod (wsats_mon _ (max n1 n2) with "W") as "W"; first lia.
+    iMod (wsats_mon _ (max n1 n2) with "W2") as "W2"; first lia.
+    iApply "SIM"; iFrame. rewrite ownE_op //; iFrame "E E2".
+    iPoseProof (wsats_merge with "[W W2]") as "$"; iFrame.
   Qed.
+    (* iApply ("SIM" with "Q"); rewrite /wsim_ginv. *)
+  (* Qed. *)
 
-  Lemma wsim_full_assume_src (P P' : iProp Σ) r g k_s i_t E :
+  (* Lemma wsim_full_assume_src (P P' : iProp Σ) r g k_s i_t E :
     ((P -∗ (wsim_ginv υ E ∗ P')) ∗
-    (P' -∗ wsim (Some true) υ ν E r g R_s R_t RR true pt nths
+    (P' -∗ wsim (Some true) υ ν E r g RR true pt nths
       (st_s, k_s tt) (st_t, i_t))) ⊢
-    wsim None υ ν E r g R_s R_t RR ps pt nths
+    wsim None υ ν E r g RR ps pt nths
       (st_s, trigger (Assume P) >>= k_s) (st_t, i_t).
   Proof using.
     unseal; iIntros "[P SIM] I". iApply isim_assume_src; eauto.
     iIntros "P'". iPoseProof ("P" with "P'") as "[GINV P]".
     iApply ("SIM" with "P GINV").
-  Qed.
+  Qed. *)
 
-  Lemma wsim_full_assume_src_upd (P P' : iProp Σ) r g k_s i_t E :
-    ((P ==∗ (wsim_ginv υ E ∗ P')) ∗
-    (P' ==∗ wsim (Some true) υ ν E r g R_s R_t RR true pt nths
-      (st_s, k_s tt) (st_t, i_t))) ⊢
-    wsim None υ ν E r g R_s R_t RR ps pt nths
-      (st_s, trigger (Assume P) >>= k_s) (st_t, i_t).
+  (* Lemma wsim_full_assume_src (P P' : iProp Σ) k_s i_t E :
+    ((P ==∗ (wsim_ginv (Some (E, E)) ∗ P')) ∗
+    (P' ==∗ sim (Some (E, E)) r g RR true pt nths (st_s, k_s tt) (st_t, i_t))) ⊢
+    sim None r g RR ps pt nths (st_s, trigger (Assume P) >>= k_s) (st_t, i_t).
   Proof using.
     unseal; iIntros "[P SIM] I". iApply isim_assume_src; eauto.
     iIntros "P'". iPoseProof ("P" with "P'") as ">[GINV P]".
-    iPoseProof ("SIM" with "P") as ">SIM".
-    iApply ("SIM" with "GINV").
-  Qed.
+    iPoseProof ("SIM" with "P") as ">SIM". iApply ("SIM" with "GINV").
+  Qed. *)
 
-  Lemma wsim_full_assume_tgt_WP `{i : !WP P υ E} r g i_s k_t :
-    (WP_remainder i ∗
-    wsim None υ ν E r g R_s R_t RR ps true nths
-      (st_s, i_s) (st_t, k_t tt)) ⊢
-    wsim (Some true) υ ν E r g R_s R_t RR ps pt nths
-      (st_s, i_s) (st_t, trigger (Assume P) >>= k_t).
+  Lemma wsim_assume_tgt_WP `{i : !WP P Ew' E'} i_s k_t Ew E :
+    Ew' ⊆ Ew → E' ⊆ E →
+    (WP_remainder i ∗ sim (Some (Ew ∖ Ew', E ∖ E')) r g RR ps true nths (st_s, i_s) (st_t, k_t tt)) ⊢
+    sim (Some (Ew, E)) r g RR ps pt nths (st_s, i_s) (st_t, trigger (Assume P) >>= k_t).
   Proof using.
-    unseal; iIntros "[P SIM] I". iApply isim_assume_tgt; eauto.
-    iSplitR "SIM"; iFrame.
+    unseal; iIntros (??) "[P SIM] [O [E [%n W]]]".
+    iMod (own_admin_split with "O") as "[O1 O2]". iApply isim_assume_tgt; eauto.
+    rewrite /wsim_ginv {2}(union_difference_L Ew' Ew) // wsats_split; last set_solver.
+    rewrite {2}(union_difference_L E' E) // ownE_op; last set_solver.
+    iDestruct "W" as "[W1 W2]"; iDestruct "E" as "[E1 E2]".
+    iSplitR "SIM E2 W2 O2".
     { iApply WP_iff; iFrame. }
-    { iApply "SIM"; done. }
+    { iApply "SIM"; iFrame. }
   Qed.
 
-  Lemma wsim_full_assume_precise_tgt_WP P `{i : !WP P υ E} r g i_s k_t :
+  (* Lemma wsim_full_assume_precise_tgt_WP P `{i : !WP P υ E} r g i_s k_t :
     (precise P -∗
-      WP_remainder i ∗
-      wsim None υ ν E r g R_s R_t RR ps true nths
-      (st_s, i_s) (st_t, k_t tt)) ⊢
-    wsim (Some true) υ ν E r g R_s R_t RR ps pt nths
+      WP_remainder i ∗ wsim None υ ν E r g RR ps true nths (st_s, i_s) (st_t, k_t tt)) ⊢
+    wsim (Some true) υ ν E r g RR ps pt nths
       (st_s, i_s) (st_t, trigger (AssumePrecise P) >>= k_t).
   Proof using.
     unseal; iIntros "H I". iApply isim_assume_precise_tgt; eauto.
@@ -551,26 +516,37 @@ Section wsim.
     iSplitR "H"; iFrame.
     { iApply WP_iff; iFrame. }
     { iApply "H". et. }
-  Qed.
-
-  Lemma wsim_full_guarantee_tgt_WP `{i : !WP P υ E} r g i_s k_t :
-    (WP_remainder i -∗
-    wsim (Some true) υ ν E r g R_s R_t RR ps true nths
-      (st_s, i_s) (st_t, k_t tt)) ⊢
-    wsim None υ ν E r g R_s R_t RR ps pt nths
-      (st_s, i_s) (st_t, trigger (Guarantee P) >>= k_t).
+  Qed. *)
+  Lemma wsim_guarantee_tgt_WP `{i : !WP P Ew' E'} i_s k_t :
+    let Ep' :=
+      match Ep with | Some (Ew, E) => Some (Ew ∪ Ew', E ∪ E') | None => Some (Ew', E') end
+    in
+    (WP_remainder i -∗ sim Ep' r g RR ps true nths (st_s, i_s) (st_t, k_t tt)) ⊢
+    sim Ep r g RR ps pt nths (st_s, i_s) (st_t, trigger (Guarantee P) >>= k_t).
   Proof using.
-    unseal. iIntros "SIM I".
-    iApply isim_guarantee_tgt; iIntros "P"; iPoseProof (WP_iff with "P") as "[P1 P2]".
-    iSpecialize ("SIM" with "P2 P1").
-    iApply "SIM"; iFrame.
+    s; iIntros "SIM"; iApply wsim_guarantee_tgt; iIntros "P".
+    iPoseProof (WP_iff i with "P") as "[P1 P2]".
+    unseal; iIntros "I".
+    iAssert ( |==> wsim_ginv
+      (match Ep with
+      | Some (Ew, E) => Some (Ew ∪ Ew', E ∪ E')
+      | None => Some (Ew', E')
+      end))%I with "[I P1]" as "> I".
+    { destruct Ep as [[??]|]; ss.
+      iDestruct "I" as "[$ [E1 [%n1 W1]]]"; iDestruct "P1" as "[_ [E2 [%n2 W2]]]".
+      iPoseProof (ownE_exploit with "[E1 E2]") as "%"; first iFrame; rewrite ownE_op //; iFrame.
+      iMod (wsats_mon _ (max n1 n2) with "W1") as "W1"; first lia.
+      iMod (wsats_mon _ (max n1 n2) with "W2") as "W2"; first lia.
+      iPoseProof (wsats_merge with "[W1 W2]") as "$"; iFrame; ss.
+    }
+    iApply ("SIM" with "P2"); ss.
   Qed.
 
-  Lemma wsim_half_assume_tgt_WP `{i : !WP P ν ⊤, υ > ν} r g i_s k_t E :
+  (* Lemma wsim_half_assume_tgt_WP `{i : !WP P ν ⊤, υ > ν} r g i_s k_t E :
     (WP_remainder i ∗
-    wsim (Some false) υ ν E r g R_s R_t RR ps true nths
+    wsim (Some false) υ ν E r g RR ps true nths
       (st_s, i_s) (st_t, k_t tt)) ⊢
-    wsim (Some true) υ ν E r g R_s R_t RR ps pt nths
+    wsim (Some true) υ ν E r g RR ps pt nths
       (st_s, i_s) (st_t, trigger (Assume P) >>= k_t).
   Proof using.
     unseal; iIntros "[P SIM] I".
@@ -585,9 +561,9 @@ Section wsim.
   Lemma wsim_half_assume_precise_tgt_WP P `{i : !WP P ν ⊤, υ > ν} r g i_s k_t E :
     (precise P -∗
        WP_remainder i ∗
-       wsim (Some false) υ ν E r g R_s R_t RR ps true nths
+       wsim (Some false) υ ν E r g RR ps true nths
          (st_s, i_s) (st_t, k_t tt)) ⊢
-    wsim (Some true) υ ν E r g R_s R_t RR ps pt nths
+    wsim (Some true) υ ν E r g RR ps pt nths
       (st_s, i_s) (st_t, trigger (AssumePrecise P) >>= k_t).
   Proof using.
     unseal; iIntros "H I".
@@ -601,9 +577,9 @@ Section wsim.
   
   Lemma wsim_half_guarantee_tgt_WP `{i : !WP P ν ⊤, υ > ν} r g i_s k_t E :
     (WP_remainder i -∗
-    wsim (Some true) υ ν E r g R_s R_t RR ps true nths
+    wsim (Some true) υ ν E r g RR ps true nths
       (st_s, i_s) (st_t, k_t tt)) ⊢
-    wsim (Some false) υ ν E r g R_s R_t RR ps pt nths
+    wsim (Some false) υ ν E r g RR ps pt nths
       (st_s, i_s) (st_t, trigger (Guarantee P) >>= k_t).
   Proof using.
     unseal. iIntros "SIM I".
@@ -611,34 +587,28 @@ Section wsim.
     iSpecialize ("SIM" with "P2").
     iDestruct "I" as "[O [W I]]". iPoseProof ("I" with "P1") as "> I".
     iApply "SIM"; iFrame.
-  Qed.
+  Qed. *)
 
   (* Derived lemmas *)
-  Lemma wsim_unwrapU_src r g X (x : option X) k_s i_t E :
-    (∀ x', ⌜x = Some x'⌝ -∗
-    wsim t υ ν E r g R_s R_t RR ps pt nths
-      (st_s, k_s x') (st_t, i_t)) ⊢
-    wsim t υ ν E r g R_s R_t RR ps pt nths
-      (st_s, unwrapU x >>= k_s) (st_t, i_t).
+  Lemma wsim_unwrapU_src X (x : option X) k_s i_t :
+    (∀ x', ⌜x = Some x'⌝ -∗ sim Ep r g RR ps pt nths (st_s, k_s x') (st_t, i_t)) ⊢
+    sim Ep r g RR ps pt nths (st_s, unwrapU x >>= k_s) (st_t, i_t).
   Proof using.
     iIntros "H". unfold unwrapU. destruct x.
     { hred_l. iApply "H". auto. }
     { unseal; iIntros "P". iApply isim_triggerUB_src. }
   Qed.
 
-  Lemma wsim_unwrapN_src r g X (x : option X) k_s i_t E :
-    (∃ x', ⌜x = Some x'⌝ ∗
-      wsim t υ ν E r g R_s R_t RR ps pt nths
-        (st_s, k_s x') (st_t, i_t)) ⊢
-    wsim t υ ν E r g R_s R_t RR ps pt nths
-      (st_s, unwrapN x >>= k_s) (st_t, i_t).
+  Lemma wsim_unwrapN_src X (x : option X) k_s i_t :
+    (∃ x', ⌜x = Some x'⌝ ∗ sim Ep r g RR ps pt nths (st_s, k_s x') (st_t, i_t)) ⊢
+    sim Ep r g RR ps pt nths (st_s, unwrapN x >>= k_s) (st_t, i_t).
   Proof using. iIntros "H". iDestruct "H" as (x') "[% H]". subst. hred_l. iApply "H". Qed.
 
-  Lemma wsim_sput_src_sandbox mask scopes k v r g k_s i_t E :
+  Lemma wsim_sput_src_sandbox mask scopes k v k_s i_t :
     In k.1 scopes →
-    wsim t υ ν E r g R_s R_t RR true pt nths
+    sim Ep r g RR true pt nths
       (alist_upd k v st_s, k_s tt) (st_t, i_t) ⊢
-    wsim t υ ν E r g R_s R_t RR ps pt nths
+    sim Ep r g RR ps pt nths
       (st_s, HModTr.sandbox mask scopes (trigger (SPut k v)) >>= k_s) (st_t, i_t).
   Proof using.
     intros IN; iIntros "SIM".
@@ -651,11 +621,11 @@ Section wsim.
     }
   Qed.
 
-  Lemma wsim_sget_src_sandbox mask scopes k r g k_s i_t E :
+  Lemma wsim_sget_src_sandbox mask scopes k k_s i_t :
     In k.1 scopes →
-    wsim t υ ν E r g R_s R_t RR true pt nths
+    sim Ep r g RR true pt nths
       (st_s, k_s (or_else (alist_find k st_s) tt↑)) (st_t, i_t) ⊢
-    wsim t υ ν E r g R_s R_t RR ps pt nths
+    sim Ep r g RR ps pt nths
       (st_s, HModTr.sandbox mask scopes (trigger (SGet k)) >>= k_s) (st_t, i_t).
   Proof using.
     intros IN; iIntros "SIM".
@@ -668,11 +638,11 @@ Section wsim.
     }
   Qed.
 
-  Lemma wsim_sput_tgt_sandbox mask scopes k v r g i_s k_t E :
+  Lemma wsim_sput_tgt_sandbox mask scopes k v i_s k_t :
     In k.1 scopes →
-    wsim t υ ν E r g R_s R_t RR ps true nths
+    sim Ep r g RR ps true nths
       (st_s, i_s) (alist_upd k v st_t, k_t tt) ⊢
-    wsim t υ ν E r g R_s R_t RR ps pt nths
+    sim Ep r g RR ps pt nths
       (st_s, i_s) (st_t, HModTr.sandbox mask scopes (trigger (SPut k v)) >>= k_t).
   Proof using.
     intros IN; iIntros "SIM".
@@ -685,11 +655,11 @@ Section wsim.
     }
   Qed.
 
-  Lemma wsim_sget_tgt_sandbox mask scopes k r g i_s k_t E :
+  Lemma wsim_sget_tgt_sandbox mask scopes k i_s k_t :
     In k.1 scopes →
-    wsim t υ ν E r g R_s R_t RR ps true nths
+    sim Ep r g RR ps true nths
       (st_s, i_s) (st_t, k_t (or_else (alist_find k st_t) tt↑)) ⊢
-    wsim t υ ν E r g R_s R_t RR ps pt nths
+    sim Ep r g RR ps pt nths
       (st_s, i_s) (st_t, HModTr.sandbox mask scopes (trigger (SGet k)) >>= k_t).
   Proof using.
     intros IN; iIntros "SIM".
@@ -702,85 +672,79 @@ Section wsim.
     }
   Qed.
 
-  Lemma wsim_asm_src (P : Prop) r g k_s i_t E :
-    (∀ _ : P, (wsim t υ ν E r g R_s R_t RR true pt nths
-      (st_s, k_s tt) (st_t, i_t))) ⊢
-    wsim t υ ν E r g R_s R_t RR ps pt nths
-      (st_s, assume P >>= k_s) (st_t, i_t).
+  Lemma wsim_asm_src (P : Prop) k_s i_t :
+    (⌜P⌝ -∗ (sim Ep r g RR true pt nths (st_s, k_s tt) (st_t, i_t))) ⊢
+    sim Ep r g RR ps pt nths (st_s, assume P >>= k_s) (st_t, i_t).
   Proof using.
     unseal; iIntros "RR I". iApply isim_asm_src; eauto.
     iIntros "%H"; iApply ("RR" $! H with "I"); iFrame.
   Qed.
 
-  Lemma wsim_asm_tgt (P : Prop) r g i_s k_t E :
-    P →
-    wsim t υ ν E r g R_s R_t RR ps true nths
-      (st_s, i_s) (st_t, k_t tt) ⊢
-    wsim t υ ν E r g R_s R_t RR ps pt nths
-      (st_s, i_s) (st_t, assume P >>= k_t).
+  Lemma wsim_asm_tgt (P : Prop) i_s k_t :
+    ⌜P⌝ ∗ sim Ep r g RR ps true nths (st_s, i_s) (st_t, k_t tt) ⊢
+    sim Ep r g RR ps pt nths (st_s, i_s) (st_t, assume P >>= k_t).
   Proof using.
-    intros H; unseal; iIntros "P I". iApply isim_asm_tgt; eauto. iApply ("P" with "I").
+    unseal; iIntros "[%HP SIM] I". iApply isim_asm_tgt; eauto. iApply ("SIM" with "I").
   Qed.
 
-  Lemma wsim_guar_src (P : Prop) r g k_s i_t E :
-    ⌜P⌝ ∗
-    wsim t υ ν E r g R_s R_t RR true pt nths
-      (st_s, k_s tt) (st_t, i_t) ⊢
-    wsim t υ ν E r g R_s R_t RR ps pt nths
-      (st_s, guarantee P >>= k_s) (st_t, i_t).
+  Lemma wsim_guar_src (P : Prop) k_s i_t :
+    ⌜P⌝ ∗ sim Ep r g RR true pt nths (st_s, k_s tt) (st_t, i_t) ⊢
+    sim Ep r g RR ps pt nths (st_s, guarantee P >>= k_s) (st_t, i_t).
   Proof using.
     unseal; iIntros "[P H] I". iApply isim_guar_src; eauto. iFrame.
     iApply ("H" with "I").
   Qed.
 
-  Lemma wsim_guar_tgt (P : Prop) r g i_s k_t E :
-    (∀ _ : P, wsim t υ ν E r g R_s R_t RR ps true nths
-      (st_s, i_s) (st_t, k_t tt)) ⊢
-    wsim t υ ν E r g R_s R_t RR ps pt nths
-      (st_s, i_s) (st_t, guarantee P >>= k_t).
+  Lemma wsim_guar_tgt (P : Prop) i_s k_t :
+    (⌜P⌝ -∗ sim Ep r g RR ps true nths (st_s, i_s) (st_t, k_t tt)) ⊢
+    sim Ep r g RR ps pt nths (st_s, i_s) (st_t, guarantee P >>= k_t).
   Proof using.
     unseal; iIntros "RR I". iApply isim_guar_tgt; eauto.
     iIntros "%H"; iApply ("RR" $! H with "I"); iFrame.
   Qed.
 
-  Lemma wsim_nodup E r g i_s i_t:
+  Lemma wsim_nodup i_s i_t:
     (∀ (NODS : List.NoDup (List.map fst st_s))
        (NODD : List.NoDup (List.map fst st_t)),
-     wsim t υ ν E r g R_s R_t RR ps pt nths (st_s, i_s) (st_t, i_t))
-    ⊢ wsim t υ ν E r g R_s R_t RR ps pt nths (st_s, i_s) (st_t, i_t).
+      sim Ep r g RR ps pt nths (st_s, i_s) (st_t, i_t))
+    ⊢ sim Ep r g RR ps pt nths (st_s, i_s) (st_t, i_t).
   Proof using.
     unseal; iIntros "SIM I". iApply isim_nodup; eauto.
-    iIntros (? ? ? ?). iApply "SIM"; eauto.
+    iIntros (????). iApply "SIM"; eauto.
   Qed.
   
-  Lemma wsim_fupd m E1 E2 b r g i_s i_t :
-    =|υ, m|={E2, E1}=> wsim (Some b) υ ν E1 r g R_s R_t RR ps pt nths (st_s, i_s) (st_t, i_t)
-    ⊢ wsim (Some b) υ ν E2 r g R_s R_t RR ps pt nths (st_s, i_s) (st_t, i_t).
+  Lemma wsim_fupd m Ew E1 E2 i_s i_t :
+    =|m, Ew|={E2, E1}=> sim (Some (Ew, E1)) r g RR ps pt nths (st_s, i_s) (st_t, i_t)
+    ⊢ sim (Some (Ew, E2)) r g RR ps pt nths (st_s, i_s) (st_t, i_t).
   Proof using.
-    unseal; rewrite ?{2}invariants.uPred_fupd_unseal /invariants.uPred_fupd_def.
-    iIntros "SIM P"; ss. rewrite /wsim_ginv.
-    destruct b; iDestruct "P" as "[O [H1 H2]]".
-    { iDestruct "H2" as "[%nw [WA [E [D WL]]]]". iDestruct "H1" as "[%nu U]".
-      iPoseProof (fupd_mon υ m (m `max` nw) with "SIM") as "SIM"; first lia.
-      rewrite ?invariants.uPred_fupd_unseal /invariants.uPred_fupd_def.
-      iMod (wsatl_mon υ nw (m `max` nw) with "[WL WA]") as "[WA WL]"; first lia; iFrame.
-      iPoseProof ("SIM" with "[WL E D]") as "> [WL [E [D SIM]]]"; first iFrame.
-      iApply "SIM"; iFrame.
-    }
-    { iDestruct "H1" as "[%nw [WA [E [D WL]]]]".
-      iPoseProof (fupd_mon υ m (m `max` nw) with "SIM") as "SIM"; first lia.
-      rewrite ?invariants.uPred_fupd_unseal /invariants.uPred_fupd_def.
-      iMod (wsatl_mon υ nw (m `max` nw) with "[WL WA]") as "[WA WL]"; first lia; iFrame.
-      iPoseProof ("SIM" with "[WL E D]") as "> [WL [E [D SIM]]]"; first iFrame.
-      iApply "SIM"; iFrame.
-    }
+    unseal; iIntros "SIM [O [E [%n [WA W]]]]".
+    set (nm := n `max` m).
+    iPoseProof (fupd_mon _ nm with "SIM") as "SIM"; first lia.
+    iMod (wsatl_mon n nm with "[WA W]") as "[WA W]"; first lia; iFrame.
+    rewrite invariants.uPred_fupd_unseal /invariants.uPred_fupd_def.
+    iMod ("SIM" with "[W E]") as "[W [E SIM]]"; iFrame.
+    iApply "SIM"; iFrame.
   Qed.
 
   (* Proofmode instances *)
-  Global Instance wsim_elim_upd r g P p i_s i_t E :
+  (* Global Instance from_modal_wsim_fup n Ew E1 E2 i_s i_t :
+    FromModal True modality_id
+      (=|n, Ew|={E1,E2}=> sim (Some (Ew, E2)) r g RR ps pt nths (st_s, i_s) (st_t, i_t))
+      (=|n, Ew|={E1,E2}=> sim (Some (Ew, E2)) r g RR ps pt nths (st_s, i_s) (st_t, i_t))
+      (sim (Some (Ew, E1)) r g RR ps pt nths (st_s, i_s) (st_t, i_t)) | 0.
+  Proof using.
+    rewrite /FromModal invariants.uPred_fupd_unseal /invariants.uPred_fupd_def /=.
+    unseal; iIntros (SUB) "SIM [$ E] !>".
+    rewrite (union_difference_L E2 E1) // /wsats ownE_op; last set_solver.
+    iDestruct "E" as "[$ E]".
+    iIntros "[O [E' [%n' W]]]"; iApply ("SIM" with "[-]").
+    iFrame. iApply (ownE_op with "[-]"); last iFrame; set_solver.
+  Qed. *)
+
+  Global Instance wsim_elim_upd P p i_s i_t :
     ElimModal True p false ( |==> P)%I P
-      (wsim t υ ν E r g R_s R_t RR ps pt nths (st_s, i_s) (st_t, i_t))
-      (wsim t υ ν E r g R_s R_t RR ps pt nths (st_s, i_s) (st_t, i_t)).
+      (sim Ep r g RR ps pt nths (st_s, i_s) (st_t, i_t))
+      (sim Ep r g RR ps pt nths (st_s, i_s) (st_t, i_t)).
   Proof using.
     unseal.
     unfold ElimModal. rewrite bi.intuitionistically_if_elim.
@@ -789,144 +753,116 @@ Section wsim.
     iApply ("H1" with "H0 HPRE").
   Qed.
 
-  Global Instance wpsim_elim_fupd_gen b E0 E1 E2 y r g P p i_s i_t :
+  Global Instance wsim_elim_fupd_gen Ew Ew' E0 E1 E2 n P p i_s i_t :
     ElimModal
-      (E0 ⊆ E2) p false
-      (=|υ, y|={E0, E1}=> P)
+      (E0 ⊆ E2 ∧ Ew' ⊆ Ew) p false
+      (=|n, Ew'|={E0, E1}=> P)
       P
-      (wsim (Some b) υ ν E2 r g R_s R_t RR ps pt nths (st_s, i_s) (st_t, i_t))
-      (wsim (Some b) υ ν (E1 ∪ (E2 ∖ E0)) r g R_s R_t RR ps pt nths (st_s, i_s) (st_t, i_t)) | 10.
+      (sim (Some (Ew, E2)) r g RR ps pt nths (st_s, i_s) (st_t, i_t))
+      (sim (Some (Ew, E1 ∪ (E2 ∖ E0))) r g RR ps pt nths (st_s, i_s) (st_t, i_t)) | 10.
   Proof using.
-    rewrite /ElimModal bi.intuitionistically_if_elim.
-    intros SUB. iIntros "[H0 H1]".
-    iApply (wsim_fupd y).
-    iMod "H0". iPoseProof ("H1" with "H0") as "H".
-    iModIntro. iFrame.
+    rewrite /ElimModal bi.intuitionistically_if_elim /=.
+    iIntros ([??]) "[P SIM]".
+    iApply (wsim_fupd n Ew (E1 ∪ E2 ∖ E0)). iMod "P".
+    iModIntro. iApply ("SIM" with "P").
   Qed.
 
-  Global Instance wpsim_elim_fupd_same_mask b E1 E2 n r g P p i_s i_t :
+  Global Instance elim_fupd_wsim_same_mask Ew Ew' E1 E2 n p P i_s i_t :
     ElimModal
-      (E1 ⊆ E2) p false
-      (=|υ, n|={E1}=> P)
+      (E1 ⊆ E2 ∧ Ew' ⊆ Ew) p false
+      (=|n, Ew|={E1}=> P)
       P
-      (wsim (Some b) υ ν E2 r g R_s R_t RR ps pt nths (st_s, i_s) (st_t, i_t))
-      (wsim (Some b) υ ν E2 r g R_s R_t RR ps pt nths (st_s, i_s) (st_t, i_t)).
+      (sim (Some (Ew, E2)) r g RR ps pt nths (st_s, i_s) (st_t, i_t))
+      (sim (Some (Ew, E2)) r g RR ps pt nths (st_s, i_s) (st_t, i_t)).
   Proof using.
     rewrite /ElimModal bi.intuitionistically_if_elim.
-    iIntros "%SUB [H0 H1]".
-    iApply (wsim_fupd n).
-    iMod "H0". iPoseProof ("H1" with "H0") as "H".
-    iModIntro. rewrite -union_difference_L; ss.
+    iIntros ([??]) "[> P SIM]"; rewrite -union_difference_L //; iApply ("SIM" with "P").
   Qed.
 
-  Global Instance wpsim_elim_fupd_simple b E0 E1 n r g P p i_s i_t :
+  Global Instance elim_fupd_wsim_simple Ew Ew' E0 E1 n P p i_s i_t :
     ElimModal
-      True p false
-      (=|υ, n|={E0, E1}=> P)
+      (Ew' ⊆ Ew) p false
+      (=|n, Ew'|={E0, E1}=> P)
       P
-      (wsim (Some b) υ ν E0 r g R_s R_t RR ps pt nths (st_s, i_s) (st_t, i_t))
-      (wsim (Some b) υ ν E1 r g R_s R_t RR ps pt nths (st_s, i_s) (st_t, i_t)).
+      (sim (Some (Ew, E0)) r g RR ps pt nths (st_s, i_s) (st_t, i_t))
+      (sim (Some (Ew, E1)) r g RR ps pt nths (st_s, i_s) (st_t, i_t)).
   Proof using.
     rewrite /ElimModal bi.intuitionistically_if_elim.
-    iIntros "_ [H0 H1]".
-    iApply (wsim_fupd n).
-    iMod "H0". iPoseProof ("H1" with "H0") as "H".
-    iModIntro. iFrame.
+    iIntros (?) "[> P SIM]". rewrite difference_diag_L right_id_L; iApply "SIM"; done.
   Qed.
-  
-  Global Instance wpsim_add_modal_FUpd b E n r g P i_s i_t :
-    AddModal (=|υ, n|={E}=> P)
-             P
-             (wsim (Some b) υ ν E r g R_s R_t RR ps pt nths (st_s, i_s) (st_t, i_t)).
+
+  Global Instance wpsim_add_modal_FUpd Ew E n P i_s i_t :
+    AddModal (=|n, Ew|={E}=> P) P
+             (sim (Some (Ew, E)) r g RR ps pt nths (st_s, i_s) (st_t, i_t)).
   Proof using.
     unfold AddModal. iIntros "[H0 H1]". iMod "H0". iApply ("H1" with "H0").
   Qed.
 
   (* Primitive simulation rules *)
-  Lemma wsim_init sti_s sti_t :
-    wsim None υ ν ⊤ ibot ibot R_s R_t RR ps pt nths sti_s sti_t ⊢
-    @isim Σ open fl_s fl_t Ist ibot ibot R_s R_t RR ps pt nths sti_s sti_t.
+  Lemma wsim_isim sti_s sti_t :
+    sim None r g RR ps pt nths sti_s sti_t ⊢
+    @isim Σ open fl_s fl_t Ist r g R_s R_t RR ps pt nths sti_s sti_t.
   Proof using.
-    unseal; iIntros "SIM"; ss; iPoseProof ("SIM" with "[]") as "SIM"; first done.
-    iPoseProof (isim_mono_knowledge with "SIM") as "SIM".
-    { instantiate (1:=ibot); i; iIntros "H"; rewrite /wsim_rel /ibot; destruct sti_src, sti_tgt.
-      iDestruct "H" as "[]".
-    }
-    { instantiate (1:=ibot); i; iIntros "H"; rewrite /wsim_rel /ibot; destruct sti_src, sti_tgt.
-      iDestruct "H" as "[]".
-    }
-    iFrame.
+    unseal; iIntros "SIM"; ss; iPoseProof ("SIM" with "[]") as "SIM"; done.
   Qed.
 
-  Lemma wsim_split sti_s sti_t :
-    (wsim_pre t υ ν ⊤ -∗ wsim None υ ν ⊤ ibot ibot R_s R_t RR ps pt nths sti_s sti_t) ⊢
-    wsim t υ ν ⊤ ibot ibot R_s R_t RR ps pt nths sti_s sti_t.
+  Lemma wsim_unfold Ew E sti_s sti_t :
+    (wsim_ginv (Some (Ew, E)) -∗ sim None r g RR ps pt nths sti_s sti_t) ⊢
+    sim (Some (Ew, E)) r g RR ps pt nths sti_s sti_t.
   Proof using.
-    unseal.
-    iIntros "SIM PRE"; ss. iApply ("SIM" with "PRE"). done.
+    unseal. iIntros "SIM PRE"; ss. iApply ("SIM" with "PRE"). done.
   Qed.
 
-  Lemma wsim_merge sti_s sti_t :
-    wsim_pre t υ ν ⊤ ∗ wsim t υ ν ⊤ ibot ibot R_s R_t RR ps pt nths sti_s sti_t ⊢
-    wsim None υ ν ⊤ ibot ibot R_s R_t RR ps pt nths sti_s sti_t.
+  Lemma wsim_fold Ew E sti_s sti_t :
+    wsim_ginv (Some (Ew, E)) ∗ sim (Some (Ew, E)) r g RR ps pt nths sti_s sti_t ⊢
+    sim None r g RR ps pt nths sti_s sti_t.
   Proof using.
-    unseal.
-    iIntros "[PRE SIM] _"; ss. iApply ("SIM" with "PRE").
+    unseal. iIntros "[PRE SIM] _"; ss. iApply ("SIM" with "PRE").
   Qed.
 
-  Lemma wsim_eqit_src E r g st_src st_tgt i_src0 i_src1 i_tgt
-    (EQIT: eqit eq false true i_src0 i_src1)
-    :
-    wsim t υ ν E r g R_s R_t RR ps pt nths (st_src, i_src0) (st_tgt, i_tgt)
-    ⊢ wsim t υ ν E r g R_s R_t RR ps pt nths (st_src, i_src1) (st_tgt, i_tgt).
+  Lemma wsim_eqit_src i_s0 i_s1 i_t :
+    eqit eq false true i_s0 i_s1 →
+    sim Ep r g RR ps pt nths (st_s, i_s0) (st_t, i_t) ⊢
+    sim Ep r g RR ps pt nths (st_s, i_s1) (st_t, i_t).
   Proof using.
-    rewrite wsim_eq /wsim_def /wsim_pre. des_ifs.
-    all: iIntros "sim w"; iPoseProof ("sim" with "w") as "sim";
-      iStopProof;
-      eapply isim_eqit_src; eauto.
+    rewrite wsim_eq /wsim_def.
+    iIntros (Heq) "S W"; iPoseProof ("S" with "W") as "S".
+    iStopProof; eapply isim_eqit_src; eauto.
   Qed.
 
-  Lemma wsim_eqit_tgt E r g st_src st_tgt i_src i_tgt0 i_tgt1
-    (EQIT: eqit eq false true i_tgt0 i_tgt1)
-    :
-    wsim t υ ν E r g R_s R_t RR ps pt nths (st_src, i_src) (st_tgt, i_tgt0)
-    ⊢ wsim t υ ν E r g R_s R_t RR ps pt nths (st_src, i_src) (st_tgt, i_tgt1).
+  Lemma wsim_eqit_tgt i_s i_t0 i_t1 :
+    eqit eq false true i_t0 i_t1 →
+    sim Ep r g RR ps pt nths (st_s, i_s) (st_t, i_t0) ⊢
+    sim Ep r g RR ps pt nths (st_s, i_s) (st_t, i_t1).
   Proof using.
-    rewrite wsim_eq /wsim_def /wsim_pre. des_ifs.
-    all: iIntros "sim w"; iPoseProof ("sim" with "w") as "sim";
-      iStopProof;
-      eapply isim_eqit_tgt; eauto.
+    rewrite wsim_eq /wsim_def.
+    iIntros (?) "S W"; iPoseProof ("S" with "W") as "S"; iStopProof; eapply isim_eqit_tgt; eauto.
   Qed.
-
-End lemmas. End wsim.
+End wsim.
 
 Section Proph.
   Context `{!sinvG Γ Σ α β τ _I _G}.
 
   Context (fl_s fl_t : alist string (Any.t → itree hmodE Any.t)).
   Context (Ist : nat → alist key Any.t → alist key Any.t → iProp Σ).
-
-  Local Notation wsim := (wsim fl_s fl_t Ist).
-
-  Context (t : option bool).
-  Context (υ ν : univ_id).
   Context (R_s R_t : Type).
+
+  Local Notation sim Ep r g := (wsim fl_s fl_t Ist Ep r g R_s R_t).
+
+  Context (Ep : option (coPset * coPset)).
+  Context (r g : rel).
   Context (RR : post R_s R_t).
   Context (ps pt : bool).
   Context (nths : nat).
   Context (st_s st_t : state).
-  
-  (** Precise Pre & Post conditions **)
 
-  Lemma wsim_assume_proph_src {X R} Pre (Post: _→R→_) r g k_s i_t E
-    :
+  (** Precise Pre & Post conditions **)
+  Lemma wsim_assume_proph_src {X R} Pre (Post: _ → R → _) k_s i_t :
     (∃ P Q,
-      (precise P) ∗
-      (∀ x:X, Pre x ==∗ P ∗ (∀ ret, Q ret ==∗ Post x ret)) ∗
-      (P -∗ wsim t υ ν E r g R_s R_t RR true pt nths (st_s, k_s Q) (st_t, i_t)))
-    ⊢
-    wsim t υ ν E r g R_s R_t RR ps pt nths
-      (st_s, (AssumeProph Pre Post) >>= k_s) (st_t, i_t).
+      precise P ∗
+      (∀ (x : X), Pre x ==∗ P ∗ (∀ ret, Q ret ==∗ Post x ret)) ∗
+      (P -∗ sim Ep r g RR true pt nths (st_s, k_s Q) (st_t, i_t))) ⊢
+    sim Ep r g RR ps pt nths (st_s, (AssumeProph Pre Post) >>= k_s) (st_t, i_t).
   Proof.
     rewrite wsim_eq /wsim_def.
     iIntros "[% [% [#PR [G H]]]] W".
@@ -934,15 +870,12 @@ Section Proph.
     iIntros "P". iApply ("H" with "P W").
   Qed.
 
-  Lemma wsim_assume_proph_src_advanced {X R} (Pre: X→_) Post r g k_s i_t E
-    :
+  Lemma wsim_assume_proph_src_advanced {X R} (Pre : X → _) Post k_s i_t :
     (∃ I P Q,
-      I ∗ (precise P) ∗
+      I ∗ precise P ∗
       (∀ x, ∃ T, (I ∗ Pre x -∗ □ T) ∗ ((□ T) ∗ Pre x ==∗ P ∗ (∀ ret: R, Q ret ==∗ Post x ret))) ∗
-      (I ∗ P -∗ wsim t υ ν E r g R_s R_t RR true pt nths (st_s, k_s Q) (st_t, i_t)))
-    ⊢
-    wsim t υ ν E r g R_s R_t RR ps pt nths
-      (st_s, (AssumeProph Pre Post) >>= k_s) (st_t, i_t).
+      (I ∗ P -∗ sim Ep r g RR true pt nths (st_s, k_s Q) (st_t, i_t))) ⊢
+    sim Ep r g RR ps pt nths (st_s, (AssumeProph Pre Post) >>= k_s) (st_t, i_t).
   Proof.
     rewrite wsim_eq /wsim_def.
     iIntros "[% [% [% [I [#PR [G H]]]]]] W".
@@ -950,15 +883,12 @@ Section Proph.
     iIntros "P". iApply ("H" with "P W").
   Qed.
 
-  Lemma wsim_assume_proph_src_simple {X R} Pre (Post: _→R→_) r g k_s i_t E
-    :
-    (∃ x: X, precise (Pre x) ∗
+  Lemma wsim_assume_proph_src_simple {X R} Pre (Post : _ → R → _) k_s i_t :
+    (∃ (x : X), precise (Pre x) ∗
       ∀ x', Pre x' -∗
         ⌜x' = x⌝ ∗
-        wsim t υ ν E r g R_s R_t RR true pt nths (st_s, k_s (Post x)) (st_t, i_t))
-    ⊢
-    wsim t υ ν E r g R_s R_t RR ps pt nths
-      (st_s, (AssumeProph Pre Post) >>= k_s) (st_t, i_t).
+        sim Ep r g RR true pt nths (st_s, k_s (Post x)) (st_t, i_t)) ⊢
+    sim Ep r g RR ps pt nths (st_s, (AssumeProph Pre Post) >>= k_s) (st_t, i_t).
   Proof.
     rewrite wsim_eq /wsim_def.
     iIntros "[% [#PR H]] W".
@@ -967,20 +897,15 @@ Section Proph.
     iSplit; et. iApply ("H" with "W").
   Qed.
 
-  Lemma wsim_assume_proph_tgt {X R} Pre (Post: _→R→_) r g i_s k_t E
-    :
-    (∃ x: X, Pre x
-       ∗
+  Lemma wsim_assume_proph_tgt {X R} Pre (Post : _ → R → _) i_s k_t :
+    (∃ x: X, Pre x ∗
        ∀ Q, (∀ ret, Q ret ==∗ Post x ret) -∗
-       wsim t υ ν E r g R_s R_t RR ps true nths (st_s, i_s) (st_t, k_t Q))
-    ⊢
-    wsim t υ ν E r g R_s R_t RR ps pt nths
-      (st_s, i_s) (st_t, (AssumeProph Pre Post) >>= k_t).
+       sim Ep r g RR ps true nths (st_s, i_s) (st_t, k_t Q)) ⊢
+    sim Ep r g RR ps pt nths (st_s, i_s) (st_t, (AssumeProph Pre Post) >>= k_t).
   Proof.
     rewrite wsim_eq /wsim_def.
     iIntros "[% [P H]] W".
     iApply isim_assume_proph_tgt. iExists _. iFrame.
     iIntros (?) "R". iApply ("H" with "R W").
   Qed.
-
 End Proph.
