theories/simulations/wsim/WTactics.v
@@ -10,7 +10,7 @@ Ltac _wstep_l :=
       rewrite bind_ret_l
   | [ |- environments.envs_entails _ (wsim _ _ _ _ _ _ _ _ _ _ _ _ _ _ _ (_, trigger (Take _) >>= _) _) ] =>
       let name := fresh "q" in iApply wsim_take_src; iIntros (name)
-  | [ |- environments.envs_entails _ (wsim _ _ _ _ ?υ _ _ _ _ _ _ _ _ _ _ (_, trigger (Assume ?P) >>= _) _) ] =>
+  (* | [ |- environments.envs_entails _ (wsim _ _ _ _ ?υ _ _ _ _ _ _ _ _ _ _ (_, trigger (Assume ?P) >>= _) _) ] =>
       first [
         tcsearch constr:(WP P υ ⊤)
           ltac:(fun c =>
@@ -20,7 +20,7 @@ Ltac _wstep_l :=
           unfold_precond_postcond P'; iIntrosFresh "ASM"
         end
       | unfold_precond_postcond P; iApply wsim_assume_src; iIntrosFresh "ASM"
-      ]
+      ] *)
   | [ |- environments.envs_entails _ (wsim _ _ _ _ _ _ _ _ _ _ _ _ _ _ _ (_, assume _ >>= _) _) ] =>
       let name := fresh "asm" in iApply wsim_asm_src; iIntros (name)
   | [ |- environments.envs_entails _ (wsim _ _ _ _ _ _ _ _ _ _ _ _ _ _ _ (_, (HModTr.sandbox _ _ (trigger (SPut _ _))) >>= _) _) ] =>
@@ -56,7 +56,7 @@ Ltac _wstep_r :=
       rewrite bind_ret_l
   | [ |- environments.envs_entails _ (wsim _ _ _ _ _ _ _ _ _ _ _ _ _ _ _ _ (_, trigger (Choose _) >>= _) ) ] =>
       let name := fresh "q" in iApply wsim_choose_tgt; iIntros (name)
-  | [ |- environments.envs_entails _ (wsim _ _ _ _ ?u ?ν _ _ _ _ _ _ _ _ _ _ (_, trigger (Guarantee ?P) >>= _) ) ] =>
+  (* | [ |- environments.envs_entails _ (wsim _ _ _ _ ?u ?ν _ _ _ _ _ _ _ _ _ _ (_, trigger (Guarantee ?P) >>= _) ) ] =>
       first [
         tcsearch constr:(WP P ν ⊤)
           ltac:(fun c =>
@@ -73,7 +73,7 @@ Ltac _wstep_r :=
           unfold_precond_postcond P'; iIntrosFresh "GRT"
         end
       | unfold_precond_postcond P; iApply wsim_guarantee_tgt; iIntrosFresh "GRT"
-      ]
+      ] *)
   | [ |- environments.envs_entails _ (wsim _ _ _ _ _ _ _ _ _ _ _ _ _ _ _ _ (_, guarantee _ >>= _)) ] =>
       let name := fresh "grt" in iApply wsim_guar_tgt; iIntros (name)
   | [ |- environments.envs_entails _ (wsim _ _ _ _ _ _ _ _ _ _ _ _ _ _ _ _ (_, (HModTr.sandbox _ _ (trigger (SPut _ _))) >>= _)) ] =>
@@ -116,7 +116,7 @@ Ltac _wforce_l :=
   match goal with
   | [ |- environments.envs_entails _ (wsim _ _ _ _ _ _ _ _ _ _ _ _ _ _ _ (_, trigger (Choose ?T) >>= _) _) ] =>
       iApply wsim_choose_src
-  | [ |- environments.envs_entails _ (wsim _ _ _ _ ?υ _ _ _ _ _ _ _ _ _ _ (_, trigger (Guarantee ?P) >>= _) _) ] =>
+  (* | [ |- environments.envs_entails _ (wsim _ _ _ _ ?υ _ _ _ _ _ _ _ _ _ _ (_, trigger (Guarantee ?P) >>= _) _) ] =>
       first [
         tcsearch constr:(WP P υ ⊤)
           ltac:(fun c =>
@@ -126,7 +126,7 @@ Ltac _wforce_l :=
           unfold_precond_postcond P'
         end
       | unfold_precond_postcond P; iApply wsim_guarantee_src
-      ]
+      ] *)
   | [ |- environments.envs_entails _ (wsim _ _ _ _ _ _ _ _ _ _ _ _ _ _ _ (_, trigger (AssumePrecise _) >>= _) _) ] =>
       iApply wsim_assume_precise_src; iSplit; [|iIntrosFresh "ASM"]
   | [ |- environments.envs_entails _ (wsim _ _ _ _ _ _ _ _ _ _ _ _ _ _ _ (_, unwrapN _ >>= _) _) ] =>
@@ -149,7 +149,7 @@ Ltac _wforce_r :=
   match goal with
   | [ |- environments.envs_entails _ (wsim _ _ _ _ _ _ _ _ _ _ _ _ _ _ _ _ (_, trigger (Take _) >>= _)) ] =>
       iApply wsim_take_tgt
-  | [ |- environments.envs_entails _ (wsim _ _ _ _ ?u ?ν _ _ _ _ _ _ _ _ _ _ (_, trigger (Assume ?P) >>= _)) ] =>
+  (* | [ |- environments.envs_entails _ (wsim _ _ _ _ ?u ?ν _ _ _ _ _ _ _ _ _ _ (_, trigger (Assume ?P) >>= _)) ] =>
       first [
         tcsearch constr:(WP P ν ⊤)
           ltac:(fun c =>
@@ -166,14 +166,14 @@ Ltac _wforce_r :=
           unfold_precond_postcond P'
         end
       | unfold_precond_postcond P; iApply wsim_assume_tgt
-      ]
-  | [ |- environments.envs_entails _ (wsim _ _ _ _ ?u ?ν _ _ _ _ _ _ _ _ _ _ (_, trigger (AssumePrecise ?P) >>= _)) ] =>
+      ] *)
+  (* | [ |- environments.envs_entails _ (wsim _ _ _ _ ?u ?ν _ _ _ _ _ _ _ _ _ _ (_, trigger (AssumePrecise ?P) >>= _)) ] =>
       first [
         tcsearch constr:(WP P ν ⊤)
           ltac:(fun c =>
             unshelve iApply (wsim_half_assume_precise_tgt_WP _ _ _ _ _ _ _ _ _ _ _ _ _ _ _ _ _ (i:=c)); [..|iIntrosFresh "PRECISE"]; eauto);
-        match goal with
-        | [ |- environments.envs_entails _ (?P' ∗ _)] =>
+            | [ |- environments.envs_entails _ (?P' ∗ _)] =>
+            match goal with
           unfold_precond_postcond P'
         end
       | tcsearch constr:(WP P u ⊤)
@@ -184,7 +184,7 @@ Ltac _wforce_r :=
           unfold_precond_postcond P'
         end
       | unfold_precond_postcond P; iApply wsim_assume_precise_tgt; iIntrosFresh "PRECISE"
-      ]
+      ] *)
   | [ |- environments.envs_entails _ (wsim _ _ _ _ _ _ _ _ _ _ _ _ _ _ _ _ (_, AssumeProph _ _ >>= _)) ] =>
       iApply wsim_assume_proph_tgt
   | [ |- environments.envs_entails _ (wsim _ _ _ _ _ _ _ _ _ _ _ _ _ _ _ _ (_, assume _ >>= _)) ] =>
@@ -234,8 +234,8 @@ Ltac wby_coind CIH :=
   iIntrosFresh "I";
   iApply CIH.
 
-Ltac winit_simF u_src u_tgt :=
-  initialize_simF; iApply (wsim_init _ _ _ u_src u_tgt).
+Ltac winit_simF :=
+  initialize_simF; iApply wsim_isim.
 
 (** Special Tactics for AssumeProph in Source **)
 
